work in progress

coq/Properties/Synthesis.v
@@ -37,41 +37,67 @@ Section SynthesisCorrectness.
 
   (* ====== Abbreviations ====== *)
   Local Notation sched_ctx := (tf_sched_ctx tf_ctx).
+  Opaque tf_sched_ctx.
   
   Local Notation spec_states := (tfs_states (tf_sched_ctx tf_ctx)).
+  Opaque tfs_states.
   Local Notation spec_states_fin := (tfs_states_fin (tf_sched_ctx tf_ctx)).
+  Opaque tfs_states_fin.
   Local Notation spec_states_size := (tfs_states_size (tf_sched_ctx tf_ctx)).
+  Opaque tfs_states_size.
   Local Notation spec_states_t := (tf_states_type spec_states_size).
+  Opaque tf_states_type.
   Local Notation spec_states_init := (tfs_states_init (tf_sched_ctx tf_ctx)).
+  Opaque tfs_states_init.
   Local Notation spec_all_states := (@finite_elements spec_states spec_states_fin).
+  Opaque finite_elements.
   Local Notation spec_state_index := (@finite_index spec_states spec_states_fin).
+  Opaque finite_index.
   Local Notation spec_state_num := (Datatypes.length spec_all_states).
 
   Local Notation spec_inputs := (tfs_inputs (tf_sched_ctx tf_ctx)).
+  Opaque tfs_inputs.
   Local Notation spec_inputs_fin := (tfs_inputs_fin (tf_sched_ctx tf_ctx)).
+  Opaque tfs_inputs_fin.
   Local Notation spec_inputs_size := (tfs_inputs_size (tf_sched_ctx tf_ctx)).
+  Opaque tfs_inputs_size.
   Local Notation spec_inputs_t := (tf_inputs_type spec_inputs_size).
+  Opaque tf_inputs_type.
   Local Notation spec_all_inputs := (@finite_elements spec_inputs spec_inputs_fin).
+  Opaque finite_elements.
   Local Notation spec_input_index := (@finite_index spec_inputs spec_inputs_fin).
+  Opaque finite_index.
   Local Notation spec_input_num := (Datatypes.length spec_all_inputs).
 
   Local Notation spec_outputs := (tfs_outputs (tf_sched_ctx tf_ctx)).
+  Opaque tfs_outputs.
   Local Notation spec_outputs_fin := (tfs_outputs_fin (tf_sched_ctx tf_ctx)).
+  Opaque tfs_outputs_fin.
   Local Notation spec_outputs_size := (tfs_outputs_size (tf_sched_ctx tf_ctx)).
+  Opaque tfs_outputs_size.
   Local Notation spec_outputs_t := (tf_outputs_type spec_outputs_size).
+  Opaque tf_outputs_type.
   Local Notation spec_all_outputs := (@finite_elements spec_outputs spec_outputs_fin).
+  Opaque finite_elements.
   Local Notation spec_output_index := (@finite_index spec_outputs spec_outputs_fin).
+  Opaque finite_index.
   Local Notation spec_output_num := (Datatypes.length spec_all_outputs).
 
   Local Notation spec_action := (tfs_action (tf_sched_ctx tf_ctx)).
+  Opaque tfs_action.
   Local Notation spec_action_fin := (tfs_action_fin (tf_sched_ctx tf_ctx)).
+  Opaque tfs_action_fin.
   Local Notation spec_all_actions := (@finite_elements spec_action spec_action_fin).
+  Opaque finite_elements.
   Local Notation spec_action_index := (@finite_index spec_action spec_action_fin).
+  Opaque finite_index.
   Local Notation spec_action_num := (Datatypes.length spec_all_actions).
 
   Local Notation spec_action_reg_size := (tf_action_reg_size tf_ctx).
   Local Notation spec_action_encoding := (tf_action_encoding tf_ctx).
+  Opaque tf_action_encoding.
   Local Notation spec_action_encoding_inj := (tf_action_encoding_inj tf_ctx).
+  Opaque tf_action_encoding_inj.
 
   Local Notation spec_schedule := (tfs_schedule (tf_sched_ctx tf_ctx)).
   Local Notation spec_done_state := (tfs_done_signal (tf_sched_ctx tf_ctx)).
@@ -81,6 +107,7 @@ Section SynthesisCorrectness.
 
   Local Notation reg_t := (@_reg_t spec_states spec_inputs spec_outputs).
   Local Notation reg_t_finite := (@_reg_t_finite tf_ctx).
+  Opaque _reg_t_finite.
   Local Notation ext_fn_t := (@_ext_fn_t spec_inputs spec_outputs).
 
   Local Notation st_env := (ContextEnv.(env_t) (tf_states_type spec_states_size)).
@@ -133,6 +160,38 @@ Section SynthesisCorrectness.
       end
   end.
 
+  Ltac extract_match_term_lhs :=
+  match goal with
+  | |- ?LHS = _ => 
+      match LHS with
+      | context [match ?X with _ => _ end] =>
+          match X with
+          | context [match _ with _ => _ end] => 
+              fail 1
+          | _ => 
+              let MT := fresh "MT" in
+              let HeqMT := fresh "HeqMT" in
+              remember X as MT eqn:HeqMT
+          end
+      end
+  end.
+
+  Ltac extract_match_term_rhs :=
+  match goal with
+  | |- _ = ?RHS => 
+      match RHS with
+      | context [match ?X with _ => _ end] =>
+          match X with
+          | context [match _ with _ => _ end] => 
+              fail 1
+          | _ => 
+              let MT := fresh "MT" in
+              let HeqMT := fresh "HeqMT" in
+              remember X as MT eqn:HeqMT
+          end
+      end
+  end.
+
   Ltac in_match_term tac :=
   match goal with
   | |- context [match ?X with _ => _ end] =>
@@ -146,6 +205,12 @@ Section SynthesisCorrectness.
           tac HeqMT;
           subst MT
       end
+  end.
+
+  Ltac let_to_projs :=
+  repeat match goal with
+  | |- context [ match ?p with (x, y) => _ end ] =>
+      rewrite (surjective_pairing p); simpl
   end.
 
   (* ====== Input Helper Lemmas ====== *)
@@ -192,20 +257,32 @@ Section SynthesisCorrectness.
     intro. rewrite in_map_iff in H. destruct H as [x [Heq Hin]]. congruence.
   Qed.
 
-  Lemma not_in_reg_ready_all_outputs:
-    ~ In (tf_ready (states_var:=spec_states) (inputs_var:=spec_inputs) (outputs_var:=spec_outputs)) (map tf_out spec_all_outputs).
-  Proof.
-    intro. rewrite in_map_iff in H. destruct H as [x [Heq Hin]]. congruence.
-  Qed.  
-
   Lemma not_in_reg_cmd_all_states:
     ~ In (tf_cmd (states_var:=spec_states) (inputs_var:=spec_inputs) (outputs_var:=spec_outputs)) (map tf_reg spec_all_states).
   Proof.
     intro. rewrite in_map_iff in H. destruct H as [x [Heq Hin]]. congruence.
   Qed.
 
+  Lemma not_in_reg_cmd_ack_all_states:
+    ~ In (tf_cmd_ack (states_var:=spec_states) (inputs_var:=spec_inputs) (outputs_var:=spec_outputs)) (map tf_reg spec_all_states).
+  Proof.
+    intro. rewrite in_map_iff in H. destruct H as [x [Heq Hin]]. congruence.
+  Qed.
+
+  Lemma not_in_reg_ready_all_outputs:
+    ~ In (tf_ready (states_var:=spec_states) (inputs_var:=spec_inputs) (outputs_var:=spec_outputs)) (map tf_out spec_all_outputs).
+  Proof.
+    intro. rewrite in_map_iff in H. destruct H as [x [Heq Hin]]. congruence.
+  Qed. 
+
   Lemma not_in_reg_cmd_all_outputs:
     ~ In (tf_cmd (states_var:=spec_states) (inputs_var:=spec_inputs) (outputs_var:=spec_outputs)) (map tf_out spec_all_outputs).
+  Proof.
+    intro. rewrite in_map_iff in H. destruct H as [x [Heq Hin]]. congruence.
+  Qed.
+
+  Lemma not_in_reg_cmd_ack_all_outputs:
+    ~ In (tf_cmd_ack (states_var:=spec_states) (inputs_var:=spec_inputs) (outputs_var:=spec_outputs)) (map tf_out spec_all_outputs).
   Proof.
     intro. rewrite in_map_iff in H. destruct H as [x [Heq Hin]]. congruence.
   Qed.
@@ -224,6 +301,18 @@ Section SynthesisCorrectness.
 
   Lemma not_in_reg_ready_all_inputs:
     ~ In (tf_ready (states_var:=spec_states) (inputs_var:=spec_inputs) (outputs_var:=spec_outputs)) (map tf_in spec_all_inputs).
+  Proof.
+    intro. rewrite in_map_iff in H. destruct H as [x [Heq Hin]]. congruence.
+  Qed.
+
+  Lemma not_in_reg_cmd_all_inputs:
+    ~ In (tf_cmd (states_var:=spec_states) (inputs_var:=spec_inputs) (outputs_var:=spec_outputs)) (map tf_in spec_all_inputs).
+  Proof.
+    intro. rewrite in_map_iff in H. destruct H as [x [Heq Hin]]. congruence.
+  Qed.
+
+  Lemma not_in_reg_cmd_ack_all_inputs:
+    ~ In (tf_cmd_ack (states_var:=spec_states) (inputs_var:=spec_inputs) (outputs_var:=spec_outputs)) (map tf_in spec_all_inputs).
   Proof.
     intro. rewrite in_map_iff in H. destruct H as [x [Heq Hin]]. congruence.
   Qed.
@@ -296,8 +385,6 @@ Section SynthesisCorrectness.
 
   End Encoding. 
 
-  Opaque _register_var_name.
-
   (* ====== State and Environment Relations ====== *)
 
   Definition state_matches (sys: sys_state_t) (r: ContextEnv.(env_t) R) : Prop :=
@@ -331,19 +418,18 @@ Section SynthesisCorrectness.
       (@snd (vect_cons_t bool (vect_nil_t bool)) (prod (vect bool (tf_action_reg_size tf_ctx)) unit) cmd_res) = spec_action_encoding act) /\
     (forall (x: spec_inputs), sigma (ext_input x) (Ob~1) = input x).
 
-  (* Lemma state_env_matches_comp :
+  Lemma state_env_matches_comp :
     forall sys act input r1 r2,
       state_equal r1 r2 ->
       env_equal r1 r2 ->
-      state_env_matches sys act input r1 = state_env_matches sys act input r2.
+      state_env_matches sys act input r1 <-> state_env_matches sys act input r2.
   Proof.
     intros. 
-    unfold state_equal in H. destruct H as [Hstate_eq Hout_eq].
-    unfold env_equal in H0. destruct H0 as [Hcmd_eq Hin_eq].
-    unfold state_env_matches, state_matches, env_matches. f_equal; [f_equal | f_equal].
-    (* - apply prop_ext.  *) (* Not provable without function extensionality *)
-
-  Admitted.  *)
+    unfold state_equal in H. destruct H as [H1 H2].
+    unfold env_equal in H0. destruct H0 as [H3 H4].
+    unfold state_env_matches, state_matches, env_matches.
+    repeat split; sauto.
+  Qed.
 
   (* ====== Initial State Correctness ====== *)
 
@@ -366,22 +452,25 @@ Section SynthesisCorrectness.
 
   (* ====== Translation Validation ====== *)
 
-  Arguments log_empty : simpl never.
-  Arguments log_cons : simpl never.
+  (* Arguments log_empty : simpl never.
+  Arguments log_cons : simpl never. *)
+  Opaque log_empty.
+  Opaque log_cons.
+  Opaque finite_elements.
+  Opaque finite_index.
 
   Section MayReadWrite.
 
     Local Notation may_read := (may_read (R:=R) (REnv:=REnv) (reg_t:=reg_t)).
     Local Notation may_write := (may_write (R:=R) (REnv:=REnv) (reg_t:=reg_t)).
 
+
     Lemma may_read0_implies_may_read1 :
       forall log_r idx,
         may_read log_r P0 idx = true -> may_read log_r P1 idx = true.
     Proof.
       intros log_r idx H. unfold may_read in *. apply andb_prop in H. destruct H as [H_is_write0 H_is_write1]. exact H_is_write1.
-    (* Time Qed. *)
-    Admitted. (* SPEEDUP *)
-    (* 15 seconds *)
+    Qed.
 
     Lemma may_write0_implies_may_write1 :
       forall log_r log_a idx,
@@ -389,10 +478,8 @@ Section SynthesisCorrectness.
     Proof.
       intros log_r log_a idx H. unfold may_write in *. apply andb_prop in H. destruct H as [H_cons H_is_write1].
       exact H_is_write1.
-    (* Time Qed. *)
-    Admitted. (* SPEEDUP *)
-    (* ??? seconds *)
-
+    Qed.
+    
     Definition may_read_all log_r port regs :=
       forallb (may_read log_r port) regs.
 
@@ -405,6 +492,106 @@ Section SynthesisCorrectness.
     Proof.
       intros log_r regs H. unfold may_read_all in *. rewrite forallb_forall in H. apply forallb_forall. intros x Hin.
       apply H in Hin. apply may_read0_implies_may_read1. exact Hin.
+    Qed.
+
+    Lemma may_read_log1_cons_neq :
+      forall log_r port
+             idx1 idx2 entry,
+        idx2 <> idx1 ->
+        may_read (log_cons idx1 entry log_r) port idx2
+        = may_read log_r port idx2.
+    Proof.
+      intros log_r port idx1 idx2 entry Hneq. destruct entry, kind.
+      - unfold may_read. rewrite !(SemanticProperties.log_existsb_log_cons_neq log_r idx2 idx1); try assumption; reflexivity.
+      - unfold may_read. rewrite !(SemanticProperties.log_existsb_log_cons_neq log_r idx2 idx1); try assumption; reflexivity.
+    Qed.
+
+    Lemma may_read_log1_cons_eq :
+      forall log_r prt
+             idx entry,
+        may_read (log_cons idx entry log_r) prt idx
+        = may_read log_r prt idx && 
+          match prt with
+          | P0 =>
+            negb (is_write0 (kind entry) (port entry))
+            && negb (is_write1 (kind entry) (port entry))
+          | P1 => negb (is_write1 (kind entry) (port entry))
+          end.
+    Proof.
+      intros log_r prt idx entry. destruct entry, kind.
+      - unfold may_read. rewrite !(SemanticProperties.log_existsb_log_cons_eq log_r idx).
+        destruct prt; simpl; rewrite andb_true_r; reflexivity.
+      - unfold may_read. rewrite !(SemanticProperties.log_existsb_log_cons_eq log_r idx).
+        destruct prt; simpl.
+        + destruct port; simpl; rewrite !andb_false_r; reflexivity.
+        + destruct port; simpl; [ rewrite andb_true_r | rewrite andb_false_r ]; reflexivity.
+    Qed.
+
+    Lemma may_read_all_log1_cons_neq :
+      forall log_r port regs idx entry,
+        ~ In idx regs ->
+        may_read_all (log_cons idx entry log_r) port regs
+        = may_read_all log_r port regs.
+    Proof.
+      intros log_r port regs idx entry Hnotin.
+      unfold may_read_all. apply forallb_pointwise. intros. 
+      assert (x <> idx) as Hx_neq.
+      { intros Heq. subst x. contradiction. }
+      rewrite may_read_log1_cons_neq; try assumption. reflexivity.
+    Qed.
+
+    Lemma may_write_log1_cons_neq :
+      forall log_r log_a port
+             idx1 idx2 entry,
+        idx2 <> idx1 ->
+        may_write (log_cons idx1 entry log_r) log_a port idx2
+        = may_write log_r log_a port idx2.
+    Proof.
+      intros log_r log_a port idx1 idx2 entry Hneq. destruct entry, kind.
+      + unfold may_write. rewrite !SemanticProperties.log_existsb_app.
+        rewrite !(SemanticProperties.log_existsb_log_cons_neq log_r idx2 idx1); try assumption; reflexivity.
+      + unfold may_write. rewrite !SemanticProperties.log_existsb_app.
+        rewrite !(SemanticProperties.log_existsb_log_cons_neq log_r idx2 idx1); try assumption; reflexivity.
+    Qed.
+
+    Lemma may_write_log1_cons_eq :
+      forall log_r log_a prt
+             idx entry,
+        may_write (log_cons idx entry log_r) log_a prt idx
+        = may_write log_r log_a prt idx && 
+          match prt with
+          | P0 =>
+            negb (is_read1 (kind entry) (port entry)) 
+            && negb (is_write0 (kind entry) (port entry))
+            && negb (is_write1 (kind entry) (port entry))
+          | P1 => negb (is_write1 (kind entry) (port entry))
+          end.
+    Proof.
+      intros log_r log_a prt idx entry. destruct entry, kind.
+      - unfold may_write. rewrite !SemanticProperties.log_existsb_app.
+        rewrite !(SemanticProperties.log_existsb_log_cons_eq log_r idx).
+        destruct prt; simpl.
+        + destruct port; simpl; [ rewrite andb_true_r | rewrite orb_true_r; rewrite andb_false_r ]; reflexivity.
+        + rewrite andb_true_r; reflexivity.
+      - unfold may_write. rewrite !SemanticProperties.log_existsb_app.
+        rewrite !(SemanticProperties.log_existsb_log_cons_eq log_r idx).
+        destruct prt; simpl.
+        + destruct port; simpl; rewrite !andb_false_r; rewrite orb_true_r; ring.
+        + destruct port; simpl; [ rewrite andb_true_r | rewrite orb_true_r; rewrite andb_false_r ]; reflexivity.
+    Qed.
+
+    Lemma may_write_all_log1_cons_neq :
+      forall log_r log_a port regs
+             idx entry,
+        ~ In idx regs ->
+        may_write_all (log_cons idx entry log_r) log_a port regs
+        = may_write_all log_r log_a port regs.
+    Proof.
+      intros log_r log_a port regs idx entry Hnotin.
+      unfold may_write_all. apply forallb_pointwise. intros.
+      assert (x <> idx) as Hx_neq.
+      { intros Heq. subst x. contradiction. }
+      rewrite may_write_log1_cons_neq; try assumption. reflexivity.
     Qed.
 
     Lemma may_write_log_cons_neq :
@@ -519,10 +706,86 @@ Section SynthesisCorrectness.
       split; assumption.
     Qed.
 
+    Section MayReadWriteLogEmpty.
+
+      Lemma may_read_log_empty :
+        forall port idx,
+          may_read log_empty port idx = true.
+      Proof. intros. unfold may_read. rewrite !SemanticProperties.log_existsb_empty. sauto. Qed.
+
+      Lemma may_write_log_empty :
+        forall port idx,
+          may_write log_empty log_empty port idx = true.
+      Proof. intros. unfold may_write. rewrite !SemanticProperties.log_existsb_app. rewrite !SemanticProperties.log_existsb_empty. sauto. Qed.
+
+      Lemma may_read_all_log_empty :
+        forall port regs,
+          may_read_all log_empty port regs = true.
+      Proof. intros. unfold may_read_all. rewrite forallb_forall. intros. apply may_read_log_empty. Qed.
+
+      Lemma may_write_all_log_empty :
+        forall port regs,
+          may_write_all log_empty log_empty port regs = true.
+      Proof. intros. unfold may_write_all. rewrite forallb_forall. intros. apply may_write_log_empty. Qed.
+
+    End MayReadWriteLogEmpty.
+
+    Section MayReadWriteOne.
+
+      Lemma may_read_all_one_state :
+        forall log port r,
+          may_read_all log port (map tf_reg spec_all_states) = true ->
+          may_read log port (tf_reg r) = true.
+      Proof.
+        intros log port r H. unfold may_read_all in H. rewrite forallb_forall in H. apply H. apply in_map. apply in_spec_all_states.
+      Qed.
+
+      Lemma may_read_all_one_output :
+        forall log port o,
+          may_read_all log port (map tf_out spec_all_outputs) = true ->
+          may_read log port (tf_out o) = true.
+      Proof.
+        intros log port o H. unfold may_read_all in H. rewrite forallb_forall in H. apply H. apply in_map. apply in_spec_all_outputs.
+      Qed.
+
+      Lemma may_read_all_one_input :
+        forall log port i,
+          may_read_all log port (map tf_in spec_all_inputs) = true ->
+          may_read log port (tf_in i) = true.
+      Proof.
+        intros log port i H. unfold may_read_all in H. rewrite forallb_forall in H. apply H. apply in_map. apply in_spec_all_inputs.
+      Qed.
+      
+      Lemma may_write_all_one_state :
+        forall log1 log2 port r,
+          may_write_all log1 log2 port (map tf_reg spec_all_states) = true ->
+          may_write log1 log2 port (tf_reg r) = true.
+      Proof.
+        intros log1 log2 port r H. unfold may_write_all in H. rewrite forallb_forall in H. apply H. apply in_map. apply in_spec_all_states.
+      Qed.
+
+      Lemma may_write_all_one_output :
+        forall log1 log2 port o,
+          may_write_all log1 log2 port (map tf_out spec_all_outputs) = true ->
+          may_write log1 log2 port (tf_out o) = true.
+      Proof.
+        intros log1 log2 port o H. unfold may_write_all in H. rewrite forallb_forall in H. apply H. apply in_map. apply in_spec_all_outputs.
+      Qed.
+
+      Lemma may_write_all_one_input :
+        forall log1 log2 port i,
+          may_write_all log1 log2 port (map tf_in spec_all_inputs) = true ->
+          may_write log1 log2 port (tf_in i) = true.
+      Proof.
+        intros log1 log2 port i H. unfold may_write_all in H. rewrite forallb_forall in H. apply H. apply in_map. apply in_spec_all_inputs.
+      Qed.
+
+    End MayReadWriteOne.
+
   End MayReadWrite.
 
-  Arguments may_read : simpl never.
-  Arguments may_write : simpl never.
+  Opaque may_read.
+  Opaque may_write.
   Arguments may_write_all : simpl never.
   Arguments may_read_all : simpl never.
 
@@ -570,7 +833,7 @@ Section SynthesisCorrectness.
         .
     Proof.
       intros. simpl. rewrite H. reflexivity.
-    Time Qed.
+    Qed.
 
   End Interpreting.
 
@@ -585,9 +848,9 @@ Section SynthesisCorrectness.
       let log_n := fold_left (fun log x => log_cons (tf_in x) (Write0 (sigma (ext_input x) Ob~1)) log) spec_all_inputs log2 in
       interp_action r sigma CtxEmpty log1 log_n rest.
   Proof.
-    intros r input sigma log1 log2 rest Hinput Hwr0_in.
+    intros r input sigma log1 log2 rest Hinput Hwr0_in. 
 
-    pose proof (nodup_spec_all_inputs) as H_nodup_inputs.
+    pose proof (nodup_spec_all_inputs) as H_nodup_inputs. 
     generalize dependent log2. generalize rest.
 
     induction spec_all_inputs as [| i inputs H0 ]; intros.
@@ -730,102 +993,11 @@ Section SynthesisCorrectness.
   Admitted. (* SPEEDUP *)
   (* 188 seconds *)
 
-  Program Fixpoint CtxReadVars (r: ContextEnv.(env_t) R) (regs: list reg_t) (sig: tsig var_t) (acc: tcontext sig) : 
-    tcontext (rev (map (fun r => (_register_var_name tf_ctx r, R r)) regs) ++ sig) :=
-    match regs with
-    | [] => acc
-    | reg :: rs => 
-        let k_tau := (_register_var_name tf_ctx reg, R reg) in
-        CtxReadVars r rs (k_tau :: sig) (CtxCons k_tau (r.[reg]) acc)
-    end.
-  Next Obligation.
-    rewrite <- List.app_assoc.
-    reflexivity.
-  Qed.
-
-  Arguments _Log : simpl never.
-
-
-  Lemma interp_action_read_vars_states:
-    forall r sigma tau sig
-      (rest : action R Sigma (rev (map (fun r => (_register_var_name tf_ctx r, R r)) (map tf_reg spec_all_states)) ++ sig) tau)
-      log_r log_a (ctx: tcontext (var_t:=var_t) sig),
-      may_read_all log_r P0 (map tf_reg spec_all_states) = true ->
-        match 
-          interp_action r sigma 
-            ctx 
-            log_r log_a 
-            (rule_read_vars tf_ctx (_register_var_name tf_ctx) (map tf_reg spec_all_states) rest)
-        return option (Log R REnv) with
-        | Some (l, _, _) => Some (l)
-        | None => None
-        end =
-        match 
-          interp_action r sigma 
-            (CtxReadVars r (map tf_reg spec_all_states) sig ctx) log_r 
-            (fold_left (fun log s => log_cons (tf_reg s) (LE LogRead P0 tt) log) spec_all_states log_a) rest
-        return option (Log R REnv) with
-        | Some (l, _, _) => Some (l)
-        | None => None
-        end.
-  Proof.
-    intros r sigma tau sig rest log_r log_a ctx Hrd0_st.
-
-
-    (* pose proof (nodup_spec_all_states) as H_nodup_all_states. *)
-    generalize dependent log_a. generalize dependent rest. generalize dependent tau. generalize dependent ctx. generalize dependent sig.
-
-    induction spec_all_states as [| s states H0 ]; intros.
-    - reflexivity.
-    - cbn in Hrd0_st. apply may_read_all_cons in Hrd0_st; destruct Hrd0_st as [Hrd0_s Hrd0_states].
-      specialize (H0 Hrd0_states). 
-      cbn. rewrite Hrd0_s. cbn. unfold opt_bind.
-      rewrite Common.bind_match.
-
-      rewrite H0; clear H0. clear.
-      admit. (* Dependent Type Hell *)
-      
-      (* set (e := TypedSynthesis.rule_read_vars_obligation_1 _ _ _ _ _).
-      set (e0 := CtxReadVars_obligation_1 _ _ _).
-      clearbody e e0. cbv zeta in e, e0.
-
-      dependent destruction e. dependent destruction e0.  *)
-   
-  Admitted.
-
-  Lemma interp_action_read_vars_outputs:
-    forall r sigma tau sig
-      (rest : action R Sigma (rev (map (fun r => (_register_var_name tf_ctx r, R r)) (map tf_out spec_all_outputs)) ++ sig) tau)
-      log_r log_a (ctx: tcontext (var_t:=var_t) sig),
-      may_read_all log_r P0 (map tf_out spec_all_outputs) = true ->
-        match interp_action r sigma ctx log_r log_a 
-          (rule_read_vars tf_ctx (_register_var_name tf_ctx) (map tf_out spec_all_outputs) rest)
-        return option (Log R REnv) with
-        | Some (l, _, _) => Some (l)
-        | None => None
-        end =
-        match 
-          interp_action r sigma (CtxReadVars r (map tf_out spec_all_outputs) sig ctx) log_r 
-            (fold_left (fun log s => log_cons (tf_out s) (LE LogRead P0 tt) log) spec_all_outputs log_a) rest
-        return option (Log R REnv) with
-        | Some (l, _, _) => Some (l)
-        | None => None
-        end.
-  Proof.
-    intros r sigma tau sig rest log_r log_a ctx Hrd0_out.
-
-    generalize dependent log_a. generalize dependent rest. generalize dependent tau. generalize dependent ctx. generalize dependent sig.
-
-    induction spec_all_outputs as [| s outputs H0 ]; intros.
-    - reflexivity.
-    - cbn in Hrd0_out. apply may_read_all_cons in Hrd0_out; destruct Hrd0_out as [Hrd0_s Hrd0_outputs].
-      specialize (H0 Hrd0_outputs). 
-      cbn. rewrite Hrd0_s. cbn. unfold opt_bind.
-      rewrite Common.bind_match.
-
-      rewrite H0; clear H0. clear.
-      admit. (* Dependent Type Hell *)
-  Admitted.
+  Definition inputs_are_buffered (input: input_t) (r: ContextEnv.(env_t) R) log :=
+    forall v, 
+      latest_write0 (REnv:=REnv) (R:=R) log (tf_in v) = Some (input v) 
+      \/ 
+      latest_write0 (REnv:=REnv) (R:=R) log (tf_in v) = None /\ r.[tf_in v] = input v.
 
   Fixpoint eval_expr_aux {szB}
       (expr: tf_expr) log
@@ -860,22 +1032,22 @@ Section SynthesisCorrectness.
             | tf_sub => (Bits.minus val_src1 val_src2, log_src2)
             | tf_mul => (convert (Bits.mul val_src1 val_src2), log_src2)
             | tf_cmp szC cmp_op =>
-                let (val_cmp_src1, log_cmp_src1) := (eval_expr_aux (szB:=szC) src1 log_src2 sys_state input) in
+                let (val_cmp_src1, log_cmp_src1) := (eval_expr_aux (szB:=szC) src1 log sys_state input) in
                 let (val_cmp_src2, log_cmp_src2) := (eval_expr_aux (szB:=szC) src2 log_cmp_src1 sys_state input) in
                 (
                   match cmp_op with
                   | tf_eq =>
-                      if beq_dec val_cmp_src1 val_cmp_src2 then Bits.of_nat szB 1 else Bits.of_nat szB 0
+                      if beq_dec val_cmp_src1 val_cmp_src2 then convert (Bits.of_nat 1 1) else convert (Bits.of_nat 1 0)
                   | tf_neq =>
-                      if beq_dec val_cmp_src1 val_cmp_src2 then Bits.of_nat szB 0 else Bits.of_nat szB 1
+                      if beq_dec val_cmp_src1 val_cmp_src2 then convert (Bits.of_nat 1 0) else convert (Bits.of_nat 1 1)
                   | tf_lt =>
-                      if Bits.unsigned_lt val_cmp_src1 val_cmp_src2 then Bits.of_nat szB 1 else Bits.of_nat szB 0
+                      if Bits.unsigned_lt val_cmp_src1 val_cmp_src2 then convert (Bits.of_nat 1 1) else convert (Bits.of_nat 1 0)
                   | tf_le =>
-                      if Bits.unsigned_le val_cmp_src1 val_cmp_src2 then Bits.of_nat szB 1 else Bits.of_nat szB 0
+                      if Bits.unsigned_le val_cmp_src1 val_cmp_src2 then convert (Bits.of_nat 1 1) else convert (Bits.of_nat 1 0)
                   | tf_gt =>
-                      if Bits.unsigned_gt val_cmp_src1 val_cmp_src2 then Bits.of_nat szB 1 else Bits.of_nat szB 0
+                      if Bits.unsigned_gt val_cmp_src1 val_cmp_src2 then convert (Bits.of_nat 1 1) else convert (Bits.of_nat 1 0)
                   | tf_ge =>
-                      if Bits.unsigned_ge val_cmp_src1 val_cmp_src2 then Bits.of_nat szB 1 else Bits.of_nat szB 0
+                      if Bits.unsigned_ge val_cmp_src1 val_cmp_src2 then convert (Bits.of_nat 1 1) else convert (Bits.of_nat 1 0)
                   end,
                   log_cmp_src2
                 )
@@ -888,60 +1060,599 @@ Section SynthesisCorrectness.
               eval_expr_aux then_expr log_cond sys_state input
         end.
 
+  Lemma fst_eval_expr_aux_eq_tf_eval_expr:
+    forall expr log1 sys input szB,
+      fst (eval_expr_aux (szB:=szB) expr log1 sys input) = tf_eval_expr (szB:=szB) spec_states_size spec_inputs_size spec_outputs_size expr sys input.
+  Proof.
+    intros expr log1 sys input szB.
+
+    generalize dependent szB.
+    generalize dependent log1.
+    induction expr; intros log1 szB; try reflexivity.
+    - cbn. destruct op. rewrite Common.fst_let_repackage. f_equal.
+      apply IHexpr.
+    - cbn. destruct op.
+      + let_to_projs. f_equal. f_equal. 
+        * apply IHexpr1.
+        * apply IHexpr2.
+      + let_to_projs. f_equal. f_equal. 
+        * apply IHexpr1.
+        * apply IHexpr2.
+      + let_to_projs. f_equal. f_equal. 
+        * apply IHexpr1.
+        * apply IHexpr2.
+      + let_to_projs. f_equal. f_equal. 
+        * apply IHexpr1.
+        * apply IHexpr2.
+      + let_to_projs. f_equal. f_equal.
+        * apply IHexpr1.
+        * apply IHexpr2.
+      + let_to_projs. f_equal. f_equal.
+        * apply IHexpr1.
+        * apply IHexpr2.
+      + let_to_projs. destr; match_eq; f_equal; try apply IHexpr1; try apply IHexpr2.
+    - cbn. let_to_projs. extract_match_term_lhs. extract_match_term_rhs.
+      assert (MT = MT0). 2: { rewrite H. subst. destr; try apply IHexpr2; try apply IHexpr3. }
+      subst. f_equal. apply (IHexpr1 log1 1).
+  Qed.
+
+  Lemma snd_eval_expr_aux_log_irrelevant:
+    forall expr log1 log2 sys input szB,
+      fst (eval_expr_aux (szB:=szB) expr log1 sys input) = fst (eval_expr_aux (szB:=szB) expr log2 sys input).
+  Proof.
+    intros expr log1 log2 sys input szB.
+
+    generalize dependent szB.
+    generalize dependent log2.
+    generalize dependent log1.
+    induction expr; intros log1 log2 szB; try reflexivity.
+    - cbn.
+      pose proof (IHexpr log1 log2 szB). 
+      destruct (eval_expr_aux expr log1 sys input).
+      destruct (eval_expr_aux expr log2 sys input).
+      cbn in *. subst. reflexivity.
+    - destruct op.
+      + cbn.
+        pose proof (IHexpr1 log1 log2 szB).
+        destruct (eval_expr_aux expr1 log1 sys input). cbn in *. subst.
+        destruct (eval_expr_aux expr1 log2 sys input). cbn in *. subst.
+        pose proof (IHexpr2 l l0 szB).
+        destruct (eval_expr_aux expr2 l sys input). cbn in *. subst.
+        destruct (eval_expr_aux expr2 l0 sys input). cbn in *. subst. reflexivity.
+      + cbn.
+        pose proof (IHexpr1 log1 log2 szB).
+        destruct (eval_expr_aux expr1 log1 sys input). cbn in *. subst.
+        destruct (eval_expr_aux expr1 log2 sys input). cbn in *. subst.
+        pose proof (IHexpr2 l l0 szB).
+        destruct (eval_expr_aux expr2 l sys input). cbn in *. subst.
+        destruct (eval_expr_aux expr2 l0 sys input). cbn in *. subst. reflexivity.
+      + cbn.
+        pose proof (IHexpr1 log1 log2 szB).
+        destruct (eval_expr_aux expr1 log1 sys input). cbn in *. subst.
+        destruct (eval_expr_aux expr1 log2 sys input). cbn in *. subst.
+        pose proof (IHexpr2 l l0 szB).
+        destruct (eval_expr_aux expr2 l sys input). cbn in *. subst.
+        destruct (eval_expr_aux expr2 l0 sys input). cbn in *. subst. reflexivity.
+      + cbn.
+        pose proof (IHexpr1 log1 log2 szB).
+        destruct (eval_expr_aux expr1 log1 sys input). cbn in *. subst.
+        destruct (eval_expr_aux expr1 log2 sys input). cbn in *. subst.
+        pose proof (IHexpr2 l l0 szB).
+        destruct (eval_expr_aux expr2 l sys input). cbn in *. subst.
+        destruct (eval_expr_aux expr2 l0 sys input). cbn in *. subst. reflexivity.
+      + cbn.
+        pose proof (IHexpr1 log1 log2 szB).
+        destruct (eval_expr_aux expr1 log1 sys input). cbn in *. subst.
+        destruct (eval_expr_aux expr1 log2 sys input). cbn in *. subst.
+        pose proof (IHexpr2 l l0 szB).
+        destruct (eval_expr_aux expr2 l sys input). cbn in *. subst.
+        destruct (eval_expr_aux expr2 l0 sys input). cbn in *. subst. reflexivity.
+      + cbn.
+        pose proof (IHexpr1 log1 log2 szB).
+        destruct (eval_expr_aux expr1 log1 sys input). cbn in *. subst.
+        destruct (eval_expr_aux expr1 log2 sys input). cbn in *. subst.
+        pose proof (IHexpr2 l l0 szB).
+        destruct (eval_expr_aux expr2 l sys input). cbn in *. subst.
+        destruct (eval_expr_aux expr2 l0 sys input). cbn in *. subst. reflexivity.
+      + cbn.
+        pose proof (IHexpr1 log1 log2 szB).
+        destruct (eval_expr_aux expr1 log1 sys input). cbn in *. subst.
+        destruct (eval_expr_aux expr1 log2 sys input). cbn in *. subst.
+        pose proof (IHexpr2 l l0 szB).
+        destruct (eval_expr_aux expr2 l sys input). cbn in *. subst.
+        destruct (eval_expr_aux expr2 l0 sys input). cbn in *. subst.
+        pose proof (IHexpr1 log1 log2 cmp_sz).
+        destruct (eval_expr_aux expr1 log1 sys input). cbn in *. subst.
+        destruct (eval_expr_aux expr1 log2 sys input). cbn in *. subst.
+        pose proof (IHexpr2 l3 l4 cmp_sz).
+        destruct (eval_expr_aux expr2 l3 sys input). cbn in *. subst.
+        destruct (eval_expr_aux expr2 l4 sys input). cbn in *. subst. reflexivity.
+    - cbn.
+      pose proof (IHexpr1 log1 log2 1).
+      destruct (eval_expr_aux expr1 log1 sys input). cbn in *. subst.
+      destruct (eval_expr_aux expr1 log2 sys input). cbn in *. subst.
+      destr. 
+      + apply IHexpr3.
+      + apply IHexpr2.
+  Qed.
+
+  Lemma snd_eval_expr_aux_app_log:
+    forall expr log1 log2 sys input szB,
+      snd (eval_expr_aux (szB:=szB) expr log1 sys input) ++ log2 = snd (eval_expr_aux (szB:=szB) expr (log1 ++ log2) sys input).
+  Proof.
+    intros expr log1 log2 sys input szB.
+
+    generalize dependent szB.
+    generalize dependent log2.
+    generalize dependent log1.
+    induction expr; intros log1 log2 szB; try reflexivity.
+    - cbn.
+      pose proof (IHexpr log1 log2 szB). 
+      destruct (eval_expr_aux expr log1 sys input).
+      destruct (eval_expr_aux expr (log1 ++ log2) sys input).
+      cbn in *. subst. reflexivity.
+    - destruct op.
+      + cbn.
+        pose proof (IHexpr1 log1 log2 szB).
+        destruct (eval_expr_aux expr1 (log1 ++ log2) sys input). cbn in *. subst.
+        destruct (eval_expr_aux expr1 log1 sys input). cbn in *. subst.
+        pose proof (IHexpr2 l log2 szB).
+        destruct (eval_expr_aux expr2 (l ++ log2) sys input). cbn in *. subst.
+        destruct (eval_expr_aux expr2 l sys input). cbn in *. reflexivity.
+      + cbn.
+        pose proof (IHexpr1 log1 log2 szB).
+        destruct (eval_expr_aux expr1 (log1 ++ log2) sys input). cbn in *. subst.
+        destruct (eval_expr_aux expr1 log1 sys input). cbn in *. subst.
+        pose proof (IHexpr2 l log2 szB).
+        destruct (eval_expr_aux expr2 (l ++ log2) sys input). cbn in *. subst.
+        destruct (eval_expr_aux expr2 l sys input). cbn in *. reflexivity.
+      + cbn.
+        pose proof (IHexpr1 log1 log2 szB).
+        destruct (eval_expr_aux expr1 (log1 ++ log2) sys input). cbn in *. subst.
+        destruct (eval_expr_aux expr1 log1 sys input). cbn in *. subst.
+        pose proof (IHexpr2 l log2 szB).
+        destruct (eval_expr_aux expr2 (l ++ log2) sys input). cbn in *. subst.
+        destruct (eval_expr_aux expr2 l sys input). cbn in *. reflexivity.
+      + cbn.
+        pose proof (IHexpr1 log1 log2 szB).
+        destruct (eval_expr_aux expr1 (log1 ++ log2) sys input). cbn in *. subst.
+        destruct (eval_expr_aux expr1 log1 sys input). cbn in *. subst.
+        pose proof (IHexpr2 l log2 szB).
+        destruct (eval_expr_aux expr2 (l ++ log2) sys input). cbn in *. subst.
+        destruct (eval_expr_aux expr2 l sys input). cbn in *. reflexivity.
+      + cbn.
+        pose proof (IHexpr1 log1 log2 szB).
+        destruct (eval_expr_aux expr1 (log1 ++ log2) sys input). cbn in *. subst.
+        destruct (eval_expr_aux expr1 log1 sys input). cbn in *. subst.
+        pose proof (IHexpr2 l log2 szB).
+        destruct (eval_expr_aux expr2 (l ++ log2) sys input). cbn in *. subst.
+        destruct (eval_expr_aux expr2 l sys input). cbn in *. reflexivity.
+      + cbn.
+        pose proof (IHexpr1 log1 log2 szB).
+        destruct (eval_expr_aux expr1 (log1 ++ log2) sys input). cbn in *. subst.
+        destruct (eval_expr_aux expr1 log1 sys input). cbn in *. subst.
+        pose proof (IHexpr2 l log2 szB).
+        destruct (eval_expr_aux expr2 (l ++ log2) sys input). cbn in *. subst.
+        destruct (eval_expr_aux expr2 l sys input). cbn in *. reflexivity.
+      + cbn.
+        pose proof (IHexpr1 log1 log2 szB).
+        destruct (eval_expr_aux expr1 (log1 ++ log2) sys input). cbn in *. subst.
+        destruct (eval_expr_aux expr1 log1 sys input). cbn in *. subst.
+        pose proof (IHexpr2 l log2 szB).
+        destruct (eval_expr_aux expr2 (l ++ log2) sys input). cbn in *. subst.
+        destruct (eval_expr_aux expr2 l sys input). cbn in *. subst.
+        pose proof (IHexpr1 log1 log2 cmp_sz). 
+        destruct (eval_expr_aux expr1 (log1 ++ log2) sys input). cbn in *. subst. 
+        destruct (eval_expr_aux expr1 log1 sys input). cbn in *. subst.
+        pose proof (IHexpr2 l1 log2 cmp_sz).
+        destruct (eval_expr_aux expr2 (l1 ++ log2) sys input). cbn in *. subst.
+        destruct (eval_expr_aux expr2 l1 sys input). cbn in *. subst. reflexivity.
+    - cbn.
+      pose proof (IHexpr1 log1 log2 1).
+      pose proof (snd_eval_expr_aux_log_irrelevant expr1 log1 (log1 ++ log2) sys input 1).
+      destruct (eval_expr_aux expr1 (log1 ++ log2) sys input). cbn in *. subst.
+      destruct (eval_expr_aux expr1 log1 sys input). cbn in *. subst.
+      destr.
+  Qed.
+    
+  Lemma snd_eval_expr_aux_app:
+    forall expr1 expr2 sys input szB1 szB2,
+      (snd (eval_expr_aux (szB:=szB2) expr2 [] sys input) ++ snd (eval_expr_aux (szB:=szB1) expr1 [] sys input))
+      =
+      snd (let (_, log_src1) := eval_expr_aux (szB:=szB1) expr1 [] sys input in eval_expr_aux (szB:=szB2) expr2 log_src1 sys input).
+  Proof.
+    intros expr1 expr2 sys input szB1 szB2.
+
+    generalize dependent szB2.
+    generalize dependent szB1.
+    induction expr2; intros szB1 szB2; try (destruct (eval_expr_aux expr1 [] sys input) as [val1 log1] eqn:Heval1; reflexivity).
+    - destruct op. cbn.
+      pose proof (IHexpr2 szB1 szB2).
+      destruct (eval_expr_aux expr1 [] sys input).
+      destruct (eval_expr_aux expr2 [] sys input).
+      destruct (eval_expr_aux expr2 l sys input).
+      cbn in *. subst. reflexivity.
+    - destruct op.
+      + cbn in *. 
+        pose proof (IHexpr2_1 szB1 szB2).
+        destruct (eval_expr_aux expr1 [] sys input).
+        destruct (eval_expr_aux expr2_1 [] sys input). 
+        destruct (eval_expr_aux expr2_1 l sys input). 
+        cbn in *. subst. 
+        destruct (eval_expr_aux expr2_2 l0 sys input) eqn:Eq1.
+        destruct (eval_expr_aux expr2_2 (l0 ++ l) sys input) eqn:Eq2.
+        apply (f_equal snd) in Eq1.
+        apply (f_equal snd) in Eq2.
+        cbn in *. subst. apply snd_eval_expr_aux_app_log.
+      + cbn in *. 
+        pose proof (IHexpr2_1 szB1 szB2).
+        destruct (eval_expr_aux expr1 [] sys input).
+        destruct (eval_expr_aux expr2_1 [] sys input). 
+        destruct (eval_expr_aux expr2_1 l sys input). 
+        cbn in *. subst. 
+        destruct (eval_expr_aux expr2_2 l0 sys input) eqn:Eq1.
+        destruct (eval_expr_aux expr2_2 (l0 ++ l) sys input) eqn:Eq2.
+        apply (f_equal snd) in Eq1.
+        apply (f_equal snd) in Eq2.
+        cbn in *. subst. apply snd_eval_expr_aux_app_log.
+      + cbn in *. 
+        pose proof (IHexpr2_1 szB1 szB2).
+        destruct (eval_expr_aux expr1 [] sys input).
+        destruct (eval_expr_aux expr2_1 [] sys input). 
+        destruct (eval_expr_aux expr2_1 l sys input). 
+        cbn in *. subst. 
+        destruct (eval_expr_aux expr2_2 l0 sys input) eqn:Eq1.
+        destruct (eval_expr_aux expr2_2 (l0 ++ l) sys input) eqn:Eq2.
+        apply (f_equal snd) in Eq1.
+        apply (f_equal snd) in Eq2.
+        cbn in *. subst. apply snd_eval_expr_aux_app_log.
+      + cbn in *. 
+        pose proof (IHexpr2_1 szB1 szB2).
+        destruct (eval_expr_aux expr1 [] sys input).
+        destruct (eval_expr_aux expr2_1 [] sys input). 
+        destruct (eval_expr_aux expr2_1 l sys input). 
+        cbn in *. subst. 
+        destruct (eval_expr_aux expr2_2 l0 sys input) eqn:Eq1.
+        destruct (eval_expr_aux expr2_2 (l0 ++ l) sys input) eqn:Eq2.
+        apply (f_equal snd) in Eq1.
+        apply (f_equal snd) in Eq2.
+        cbn in *. subst. apply snd_eval_expr_aux_app_log.
+      + cbn in *. 
+        pose proof (IHexpr2_1 szB1 szB2).
+        destruct (eval_expr_aux expr1 [] sys input).
+        destruct (eval_expr_aux expr2_1 [] sys input). 
+        destruct (eval_expr_aux expr2_1 l sys input). 
+        cbn in *. subst. 
+        destruct (eval_expr_aux expr2_2 l0 sys input) eqn:Eq1.
+        destruct (eval_expr_aux expr2_2 (l0 ++ l) sys input) eqn:Eq2.
+        apply (f_equal snd) in Eq1.
+        apply (f_equal snd) in Eq2.
+        cbn in *. subst. apply snd_eval_expr_aux_app_log.
+      + cbn in *. 
+        pose proof (IHexpr2_1 szB1 szB2).
+        destruct (eval_expr_aux expr1 [] sys input).
+        destruct (eval_expr_aux expr2_1 [] sys input). 
+        destruct (eval_expr_aux expr2_1 l sys input). 
+        cbn in *. subst. 
+        destruct (eval_expr_aux expr2_2 l0 sys input) eqn:Eq1.
+        destruct (eval_expr_aux expr2_2 (l0 ++ l) sys input) eqn:Eq2.
+        apply (f_equal snd) in Eq1.
+        apply (f_equal snd) in Eq2.
+        cbn in *. subst. apply snd_eval_expr_aux_app_log.
+      + cbn in *. 
+        pose proof (IHexpr2_1 szB1 szB2).
+        pose proof (IHexpr2_1 szB1 cmp_sz).
+        destruct (eval_expr_aux expr1 [] sys input).
+        destruct (eval_expr_aux expr2_1 [] sys input). 
+        destruct (eval_expr_aux expr2_1 l sys input). 
+        cbn in *. subst. 
+        destruct (eval_expr_aux expr2_2 l0 sys input) eqn:Eq1.
+        destruct (eval_expr_aux expr2_2 (l0 ++ l) sys input) eqn:Eq2.
+        destruct (eval_expr_aux expr2_1 [] sys input). 
+        destruct (eval_expr_aux expr2_1 l sys input). 
+        cbn in *. subst. 
+        destruct (eval_expr_aux expr2_2 l3 sys input) eqn:Eq5.
+        destruct (eval_expr_aux expr2_2 (l3 ++ l) sys input) eqn:Eq6.
+        apply (f_equal snd) in Eq1.
+        apply (f_equal snd) in Eq2.
+        apply (f_equal snd) in Eq5.
+        apply (f_equal snd) in Eq6.
+        cbn in *. subst.
+        apply (snd_eval_expr_aux_app_log expr2_2 _ l sys input). 
+    - cbn.
+      pose proof (IHexpr2_2 szB1 szB2).
+      pose proof (IHexpr2_3 szB1 szB2).
+      destruct (eval_expr_aux expr1 [] sys input).
+      pose proof (snd_eval_expr_aux_log_irrelevant expr2_1 [] l sys input 1).
+      destruct (eval_expr_aux expr2_1 [] sys input) eqn:Eq1.
+      destruct (eval_expr_aux expr2_1 l sys input) eqn:Eq2.
+      destruct (eval_expr_aux expr2_2 [] sys input) eqn:Eq3.
+      destruct (eval_expr_aux expr2_2 l sys input) eqn:Eq4.
+      destruct (eval_expr_aux expr2_3 [] sys input) eqn:Eq5.
+      destruct (eval_expr_aux expr2_3 l sys input) eqn:Eq6.
+      apply (f_equal snd) in Eq1.
+      apply (f_equal snd) in Eq2.
+      apply (f_equal snd) in Eq3.
+      apply (f_equal snd) in Eq4.
+      apply (f_equal snd) in Eq5.
+      apply (f_equal snd) in Eq6.
+      cbn in *. subst. destr.
+      * rewrite (snd_eval_expr_aux_app_log expr2_3 _ l sys input szB2). f_equal. f_equal.
+        rewrite (snd_eval_expr_aux_app_log expr2_1 _ l sys input 1). reflexivity.
+      * rewrite (snd_eval_expr_aux_app_log expr2_2 _ l sys input szB2). f_equal. f_equal.
+        rewrite (snd_eval_expr_aux_app_log expr2_1 _ l sys input 1). reflexivity.
+  Qed. 
+
+  Lemma snd_eval_expr_aux_app2:
+    forall expr1 expr2 sys input szB1 szB2,
+      (snd (eval_expr_aux (szB:=szB2) expr2 [] sys input) ++ snd (eval_expr_aux (szB:=szB1) expr1 [] sys input))
+      =
+      snd (eval_expr_aux (szB:=szB2) expr2 (snd (eval_expr_aux (szB:=szB1) expr1 [] sys input)) sys input).
+  Proof.
+    intros expr1 expr2 sys input szB1 szB2.
+    rewrite snd_eval_expr_aux_app. 
+    destruct (eval_expr_aux expr1 [] sys input) as [val1 log1] eqn:Heval1.
+    apply (f_equal snd) in Heval1. cbn in Heval1. subst log1. 
+    reflexivity.
+  Qed.
+
   Definition expr_log (expr: tf_expr) (szB: nat) (sys_state: sys_state_t) (input: input_t) log :=
-    fold_left (fun acc reg => log_cons (R:=R) (REnv:=REnv) reg {| kind := LogRead; port := match reg with
+    fold_right (fun reg acc => log_cons (R:=R) (REnv:=REnv) reg {| kind := LogRead; port := match reg with
                                                    | tf_in v => P1
                                                    | _ => P0
-                                                   end; val := tt |} acc ) (snd (eval_expr_aux (szB:=szB) expr [] sys_state input)) log.
+                                                   end; val := tt |} acc ) log (snd (eval_expr_aux (szB:=szB) expr [] sys_state input)).
+   
+  Lemma latest_write0_expr_log :
+    forall expr szB sys input log_a v,
+      latest_write0 (expr_log expr szB sys input log_a) (tf_in v) =
+      latest_write0 log_a (tf_in v).
+  Proof.
+    intros expr szB sys input log_a v.
 
-  (* 
-  TODO: here
-  
+    unfold expr_log.
+    induction ((snd (eval_expr_aux expr [] sys input))).
+    - reflexivity.
+    - destruct (eq_dec (tf_in v) a) as [Heq | Hneq]; subst.
+      + simpl. rewrite SemanticProperties.latest_write0_cons_eq. exact IHl.
+      + simpl. rewrite SemanticProperties.latest_write0_cons_neq; try assumption.
+  Qed.
+
+  Lemma inputs_are_buffered_expr_log :
+    forall input r log_a log_r expr szB sys,
+      inputs_are_buffered input r (log_app log_a log_r) ->
+      inputs_are_buffered input r (log_app (expr_log expr szB sys input log_a) log_r).
+  Proof.
+    intros input r log_a log_r expr szB sys Hlatest.
+    unfold inputs_are_buffered in *. intros v. specialize (Hlatest v).
+    rewrite SemanticProperties.latest_write0_app in *.
+    rewrite latest_write0_expr_log. exact Hlatest.
+  Qed.
+
   Lemma interp_synth_convert :
-    forall r sigma log_r log_a szA ctx sig szB (expr : action R Sigma sig (bits_t szA)),
-      interp_action (R:=R) (REnv:=REnv) r sigma ctx log_r log_a (synth_convert (in_var_size := szA) tf_ctx szB expr) = 
-      match interp_action (R:=R) (REnv:=REnv) r sigma ctx log_r log_a expr 
-      return option (Log R REnv * bits_t szB * sig) with
+    forall r sigma log_r log_a szA szB (expr : action R Sigma _ (bits_t szA)),
+      interp_action (R:=R) (REnv:=REnv) r sigma CtxEmpty log_r log_a (synth_convert (in_var_size := szA) tf_ctx szB expr) = 
+      match 
+        interp_action (R:=R) (REnv:=REnv) r sigma CtxEmpty log_r log_a expr 
+      return option (Log R REnv * bits_t szB * _) with
       | Some (l, v, g) => Some (l, convert (szB:=szB) v, g)
       | None => None
       end.
   Proof.
-    intros r sigma log_r log_a szB szA expr.
+    intros r sigma log_r log_a szA szB expr.
 
-    unfold synth_convert. 
-    generalize dependent expr.
-    (* Dependent Type Hell *)
-    (* destruct (lt_eq_lt_dec szA szB) as [[Hlt | Hlt] | Hgt]; intros. *)
-    admit.
-  Admitted. *)
+    unfold synth_convert, convert.
+    destruct (eq_dec szA szB) as [Heq | Hneq]; subst.
+    - sauto.
+    - cbn. unfold opt_bind. reflexivity.
+  (* Timeout 600 Time Qed.  *)
+  Admitted. (* SPEEDUP *)
+  (* ??? seconds *)
 
   Lemma interp_action_expr :
     forall (sys: sys_state_t) (r: ContextEnv.(env_t) R) 
            (act: spec_action) (input: input_t)
            (sigma: forall f, Sig_denote (Sigma f))
-           log_r log_a expr dst,
+           log_r log_a expr dst_sz,
       state_matches sys r ->
-      env_matches act input r ->
-      interp_action r sigma
-        (CtxReadVars r (map tf_out spec_all_outputs) (rev (map (fun r0 : reg_t => (_register_var_name tf_ctx r0, R r0)) (map tf_reg spec_all_states)) ++ [])
-        (CtxReadVars r (map tf_reg spec_all_states) [] CtxEmpty)) log_r log_a (expr_to_action tf_ctx expr (spec_states_size dst))
+      may_read_all log_r P0 (map tf_reg spec_all_states) = true ->
+      may_read_all log_r P1 (map tf_in spec_all_inputs) = true ->
+      may_read_all log_r P0 (map tf_out spec_all_outputs) = true ->
+      inputs_are_buffered input r (log_app log_a log_r) ->
+      interp_action r sigma CtxEmpty log_r log_a (expr_to_action tf_ctx expr dst_sz)
       = Some (
-          expr_log expr (spec_states_size dst) sys input log_a, 
-          tf_eval_expr (szB:=spec_states_size dst) spec_states_size spec_inputs_size spec_outputs_size expr sys input, 
-          CtxReadVars r (map tf_out spec_all_outputs) (rev (map (fun r0 : reg_t => (_register_var_name tf_ctx r0, R r0)) (map tf_reg spec_all_states)) ++ [])
-          (CtxReadVars r (map tf_reg spec_all_states) [] CtxEmpty)
+          expr_log expr dst_sz sys input log_a, 
+          tf_eval_expr (szB:=dst_sz) spec_states_size spec_inputs_size spec_outputs_size expr sys input, 
+          CtxEmpty
         ).
   Proof.
-    intros sys r act input sigma log_r log_a expr dst.
-    intros Hstate Hinput_rdy.
+    intros sys r act input sigma log_r log_a expr dst_sz.
+    intros Hstate Hrd0_st Hrd1_in Hrd0_out.
 
-    induction expr.
+    unfold state_matches in Hstate. destruct Hstate as [Hstate_r Hstate_out].
+
+    generalize dependent dst_sz.
+    generalize dependent log_a.
+    induction expr; intros log_a dst_sz Hin_buf.
     + (* Const *)
       reflexivity.
     + (* Var *)
-      cbn. rewrite interp_synth_convert. reflexivity.
-      
-      admit. 
+      cbn. rewrite interp_synth_convert.
+      rewrite interp_action_read0 with (idx:=(tf_reg v)).
+      * rewrite Hstate_r. reflexivity.
+      * apply may_read_all_one_state. exact Hrd0_st.
+    + (* Input *)
+      cbn. rewrite interp_synth_convert.
+      cbn [interp_action]. rewrite may_read_all_one_input with (i:=v); try assumption.
+      unfold inputs_are_buffered, inputs_are_buffered in Hin_buf. specialize (Hin_buf v).
+      destruct Hin_buf.
+      * rewrite H. reflexivity.
+      * destruct H as [H1 H2]. rewrite H1. rewrite H2. reflexivity. 
+    + (* Output *)
+      cbn. rewrite interp_synth_convert.
+      rewrite interp_action_read0 with (idx:=(tf_out v)).
+      * rewrite Hstate_out. reflexivity.
+      * apply may_read_all_one_output. exact Hrd0_out.
+    + (* Op1 *)
+      cbn. unfold opt_bind. rewrite IHexpr; try assumption.
+      destruct op; simpl. unfold Bits.neg. f_equal. f_equal. f_equal.
+      unfold expr_log. simpl. destruct (eval_expr_aux expr [] sys input) as [val log_expr]. reflexivity.
+    + (* Op2 *)
+      destruct op.
+      - cbn. unfold opt_bind. rewrite IHexpr1; clear IHexpr1; try assumption. rewrite IHexpr2; clear IHexpr2.
+        * f_equal. f_equal. f_equal.
+          unfold expr_log. rewrite <- fold_right_app. simpl. f_equal.
+          destruct (eval_expr_aux expr1 [] sys input) as [val1 log_expr1] eqn:Eq1. 
+          destruct (eval_expr_aux expr2 log_expr1 sys input) as [val2 log_expr2] eqn:Eq2.
+          apply (f_equal snd) in Eq1. apply (f_equal snd) in Eq2. cbn in *. subst.
+          apply snd_eval_expr_aux_app2.
+        * apply inputs_are_buffered_expr_log. exact Hin_buf.
+      - cbn. unfold opt_bind. rewrite IHexpr1; clear IHexpr1; try assumption. rewrite IHexpr2; clear IHexpr2.
+        * f_equal. f_equal. f_equal.
+          unfold expr_log. rewrite <- fold_right_app. simpl. f_equal.
+          destruct (eval_expr_aux expr1 [] sys input) as [val1 log_expr1] eqn:Eq1. 
+          destruct (eval_expr_aux expr2 log_expr1 sys input) as [val2 log_expr2] eqn:Eq2.
+          apply (f_equal snd) in Eq1. apply (f_equal snd) in Eq2. cbn in *. subst.
+          apply snd_eval_expr_aux_app2.
+        * apply inputs_are_buffered_expr_log. exact Hin_buf.
+      - cbn. unfold opt_bind. rewrite IHexpr1; clear IHexpr1; try assumption. rewrite IHexpr2; clear IHexpr2.
+        * f_equal. f_equal. f_equal.
+          unfold expr_log. rewrite <- fold_right_app. simpl. f_equal.
+          destruct (eval_expr_aux expr1 [] sys input) as [val1 log_expr1] eqn:Eq1. 
+          destruct (eval_expr_aux expr2 log_expr1 sys input) as [val2 log_expr2] eqn:Eq2.
+          apply (f_equal snd) in Eq1. apply (f_equal snd) in Eq2. cbn in *. subst.
+          apply snd_eval_expr_aux_app2.
+        * apply inputs_are_buffered_expr_log. exact Hin_buf.
+      - cbn. unfold opt_bind. rewrite IHexpr1; clear IHexpr1; try assumption. rewrite IHexpr2; clear IHexpr2.
+        * f_equal. f_equal. f_equal.
+          unfold expr_log. rewrite <- fold_right_app. simpl. f_equal.
+          destruct (eval_expr_aux expr1 [] sys input) as [val1 log_expr1] eqn:Eq1. 
+          destruct (eval_expr_aux expr2 log_expr1 sys input) as [val2 log_expr2] eqn:Eq2.
+          apply (f_equal snd) in Eq1. apply (f_equal snd) in Eq2. cbn in *. subst.
+          apply snd_eval_expr_aux_app2.
+        * apply inputs_are_buffered_expr_log. exact Hin_buf.
+      - cbn. unfold opt_bind. rewrite IHexpr1; clear IHexpr1; try assumption. rewrite IHexpr2; clear IHexpr2.
+        * f_equal. f_equal. f_equal.
+          unfold expr_log. rewrite <- fold_right_app. simpl. f_equal.
+          destruct (eval_expr_aux expr1 [] sys input) as [val1 log_expr1] eqn:Eq1. 
+          destruct (eval_expr_aux expr2 log_expr1 sys input) as [val2 log_expr2] eqn:Eq2.
+          apply (f_equal snd) in Eq1. apply (f_equal snd) in Eq2. cbn in *. subst.
+          apply snd_eval_expr_aux_app2.
+        * apply inputs_are_buffered_expr_log. exact Hin_buf.
+      - cbn. rewrite interp_synth_convert.
+        cbn. rewrite IHexpr1; clear IHexpr1; try assumption. cbn. rewrite IHexpr2; clear IHexpr2.
+        * cbn. f_equal. f_equal. f_equal.
+          unfold expr_log. rewrite <- fold_right_app. simpl. f_equal.
+          destruct (eval_expr_aux expr1 [] sys input) as [val1 log_expr1] eqn:Eq1. 
+          destruct (eval_expr_aux expr2 log_expr1 sys input) as [val2 log_expr2] eqn:Eq2.
+          apply (f_equal snd) in Eq1. apply (f_equal snd) in Eq2. cbn in *. subst.
+          apply snd_eval_expr_aux_app2.
+        * apply inputs_are_buffered_expr_log. exact Hin_buf.
+      - cbn.
+        destruct cmp_op.
+        * rewrite interp_synth_convert.
+          cbn. rewrite IHexpr1; clear IHexpr1; try assumption. cbn. rewrite IHexpr2; clear IHexpr2.
+          ** cbn. f_equal. f_equal. f_equal.
+            ++ unfold expr_log. rewrite <- fold_right_app. simpl. f_equal.
+              destruct (eval_expr_aux expr1 [] sys input) as [val1 log_expr1] eqn:Eq1. 
+              destruct (eval_expr_aux expr2 log_expr1 sys input) as [val2 log_expr2] eqn:Eq2.
+              apply (f_equal snd) in Eq1. apply (f_equal snd) in Eq2. cbn in *. subst.
+              set (x1 := eval_expr_aux expr1 [] sys input) at 2. destruct x1.
+              destruct (eval_expr_aux expr2 l sys input). cbn in *. 
+              apply snd_eval_expr_aux_app2.
+            ++ unfold BitFuns._eq. destr. 
+              -- f_equal. apply beq_dec_iff in Heqb. rewrite Heqb. rewrite beq_dec_refl. reflexivity.
+              -- f_equal. f_equal. assumption.  
+          ** apply inputs_are_buffered_expr_log. exact Hin_buf.
+        * rewrite interp_synth_convert.
+          cbn. rewrite IHexpr1; clear IHexpr1; try assumption. cbn. rewrite IHexpr2; clear IHexpr2.
+          ** cbn. f_equal. f_equal. f_equal.
+            ++ unfold expr_log. rewrite <- fold_right_app. simpl. f_equal.
+              destruct (eval_expr_aux expr1 [] sys input) as [val1 log_expr1] eqn:Eq1. 
+              destruct (eval_expr_aux expr2 log_expr1 sys input) as [val2 log_expr2] eqn:Eq2.
+              apply (f_equal snd) in Eq1. apply (f_equal snd) in Eq2. cbn in *. subst.
+              set (x1 := eval_expr_aux expr1 [] sys input) at 2. destruct x1.
+              destruct (eval_expr_aux expr2 l sys input). cbn in *. 
+              apply snd_eval_expr_aux_app2.
+            ++ unfold BitFuns._neq. destr. 
+              -- f_equal. apply beq_dec_iff in Heqb. rewrite Heqb. rewrite beq_dec_refl. reflexivity.
+              -- f_equal. f_equal. rewrite negb_true_iff. assumption.  
+          ** apply inputs_are_buffered_expr_log. exact Hin_buf.
+        * rewrite interp_synth_convert.
+          cbn. rewrite IHexpr1; clear IHexpr1; try assumption. cbn. rewrite IHexpr2; clear IHexpr2.
+          ** cbn. f_equal. f_equal. f_equal.
+            ++ unfold expr_log. rewrite <- fold_right_app. simpl. f_equal.
+              destruct (eval_expr_aux expr1 [] sys input) as [val1 log_expr1] eqn:Eq1. 
+              destruct (eval_expr_aux expr2 log_expr1 sys input) as [val2 log_expr2] eqn:Eq2.
+              apply (f_equal snd) in Eq1. apply (f_equal snd) in Eq2. cbn in *. subst.
+              set (x1 := eval_expr_aux expr1 [] sys input) at 2. destruct x1.
+              destruct (eval_expr_aux expr2 l sys input). cbn in *. 
+              apply snd_eval_expr_aux_app2.
+            ++ unfold BitFuns.bitfun_of_predicate. destr. 
+          ** apply inputs_are_buffered_expr_log. exact Hin_buf.
+        * rewrite interp_synth_convert.
+          cbn. rewrite IHexpr1; clear IHexpr1; try assumption. cbn. rewrite IHexpr2; clear IHexpr2.
+          ** cbn. f_equal. f_equal. f_equal.
+            ++ unfold expr_log. rewrite <- fold_right_app. simpl. f_equal.
+              destruct (eval_expr_aux expr1 [] sys input) as [val1 log_expr1] eqn:Eq1. 
+              destruct (eval_expr_aux expr2 log_expr1 sys input) as [val2 log_expr2] eqn:Eq2.
+              apply (f_equal snd) in Eq1. apply (f_equal snd) in Eq2. cbn in *. subst.
+              set (x1 := eval_expr_aux expr1 [] sys input) at 2. destruct x1.
+              destruct (eval_expr_aux expr2 l sys input). cbn in *. 
+              apply snd_eval_expr_aux_app2.
+            ++ unfold BitFuns.bitfun_of_predicate. destr. 
+          ** apply inputs_are_buffered_expr_log. exact Hin_buf.
+        * rewrite interp_synth_convert.
+          cbn. rewrite IHexpr1; clear IHexpr1; try assumption. cbn. rewrite IHexpr2; clear IHexpr2.
+          ** cbn. f_equal. f_equal. f_equal.
+            ++ unfold expr_log. rewrite <- fold_right_app. simpl. f_equal.
+              destruct (eval_expr_aux expr1 [] sys input) as [val1 log_expr1] eqn:Eq1. 
+              destruct (eval_expr_aux expr2 log_expr1 sys input) as [val2 log_expr2] eqn:Eq2.
+              apply (f_equal snd) in Eq1. apply (f_equal snd) in Eq2. cbn in *. subst.
+              set (x1 := eval_expr_aux expr1 [] sys input) at 2. destruct x1.
+              destruct (eval_expr_aux expr2 l sys input). cbn in *. 
+              apply snd_eval_expr_aux_app2.
+            ++ unfold BitFuns.bitfun_of_predicate. destr. 
+          ** apply inputs_are_buffered_expr_log. exact Hin_buf.
+        * rewrite interp_synth_convert.
+          cbn. rewrite IHexpr1; clear IHexpr1; try assumption. cbn. rewrite IHexpr2; clear IHexpr2.
+          ** cbn. f_equal. f_equal. f_equal.
+            ++ unfold expr_log. rewrite <- fold_right_app. simpl. f_equal.
+              destruct (eval_expr_aux expr1 [] sys input) as [val1 log_expr1] eqn:Eq1. 
+              destruct (eval_expr_aux expr2 log_expr1 sys input) as [val2 log_expr2] eqn:Eq2.
+              apply (f_equal snd) in Eq1. apply (f_equal snd) in Eq2. cbn in *. subst.
+              set (x1 := eval_expr_aux expr1 [] sys input) at 2. destruct x1.
+              destruct (eval_expr_aux expr2 l sys input). cbn in *. 
+              apply snd_eval_expr_aux_app2.
+            ++ unfold BitFuns.bitfun_of_predicate. destr. 
+          ** apply inputs_are_buffered_expr_log. exact Hin_buf.
+    + (* If *)
+      cbn. unfold opt_bind. rewrite IHexpr1; try assumption.
+      destruct (tf_eval_expr spec_states_size spec_inputs_size spec_outputs_size expr1 sys input) eqn:Eq1.
+      destruct vhd eqn:Eq2; cbn in *.
+      * rewrite IHexpr2; try assumption.
+        ++ f_equal. f_equal. f_equal.
+          unfold expr_log. rewrite <- fold_right_app. simpl. f_equal.
+          let_to_projs. simpl. rewrite <- (fst_eval_expr_aux_eq_tf_eval_expr expr1 [] sys input) in Eq1.
+          subst. destruct vtl.
+          change (vect_cons_t bool (vect_nil_t bool)) with (type_denote (bits_t (S O))).
+          rewrite Eq1. simpl.
+          change (vect_cons_t bool (vect_nil_t bool)) with (type_denote (bits_t 1)).
+          apply snd_eval_expr_aux_app2.
+        ++ apply inputs_are_buffered_expr_log. exact Hin_buf.
+      * rewrite IHexpr3; try assumption.
+        ++ f_equal. f_equal. f_equal.
+          -- unfold expr_log. rewrite <- fold_right_app. simpl. f_equal.
+            let_to_projs. simpl. rewrite <- (fst_eval_expr_aux_eq_tf_eval_expr expr1 [] sys input) in Eq1.
+            subst. destruct vtl.
+            change (vect_cons_t bool (vect_nil_t bool)) with (type_denote (bits_t (S O))).
+            rewrite Eq1. simpl.
+            change (vect_cons_t bool (vect_nil_t bool)) with (type_denote (bits_t 1)).
+            apply snd_eval_expr_aux_app2.
+          -- subst. destruct vtl. reflexivity.
+        ++ apply inputs_are_buffered_expr_log. exact Hin_buf.
+  (* Timeout 10 Time Qed. *)
+  Admitted. (* SPEEDUP *)
+  (* 2 seconds *)
 
   Definition affected_regs (ops: list (@tf_op spec_states spec_inputs spec_outputs)) : list reg_t :=
     fold_right (fun op acc => match op with
@@ -950,37 +1661,146 @@ Section SynthesisCorrectness.
                              | _ => acc
                              end) [] ops.
 
+  Definition aux_log sys input (ops: list (@tf_op spec_states spec_inputs spec_outputs)) (log_a: Log R ContextEnv) : Log R ContextEnv :=
+    fold_left (fun acc op => match op with
+                             | tf_assign dst expr => log_cons (R:=R) (REnv:=REnv) (tf_reg dst) (Write0 (tf_eval_expr spec_states_size spec_inputs_size spec_outputs_size expr sys input)) (expr_log expr (spec_states_size dst) sys input acc)
+                             | tf_output dst expr => log_cons (R:=R) (REnv:=REnv) (tf_out dst) (Write0 (tf_eval_expr spec_states_size spec_inputs_size spec_outputs_size expr sys input)) (expr_log expr (spec_outputs_size dst) sys input acc)
+                             | _ => acc
+                             end) ops log_a.
+
+  Lemma inputs_are_buffered_log_app_log_cons_neq:
+    forall input r log_a log_r reg entry,
+      ~ In reg (map tf_in spec_all_inputs) ->
+      inputs_are_buffered input r (log_app log_a log_r) ->
+      inputs_are_buffered input r (log_app (log_cons (R:=R) (REnv:=REnv) reg entry log_a) log_r).
+  Proof.
+    intros input r log_a log_r reg entry Hnot_input Hin_buf.
+    unfold inputs_are_buffered in *. intros v. specialize (Hin_buf v).
+    rewrite SemanticProperties.latest_write0_app in *.
+    rewrite SemanticProperties.latest_write0_cons_neq in *; try assumption.
+    clear Hin_buf.
+    pose proof (in_spec_all_inputs v).
+    intro. subst. apply (in_map (tf_in (states_var:=spec_states) (outputs_var:=spec_outputs))) in H.
+    congruence.
+  Qed.
+
+  Lemma inputs_not_affected:
+    forall ops v,
+      ~ In (tf_in v) (affected_regs ops).
+  Proof.
+    intros ops v. unfold affected_regs. induction ops as [| op ops IH].
+    - auto.
+    - destruct op; simpl; try apply IH.
+      + (* hammer. *) timeout 10 sfirstorder.
+      + (* hammer. *) timeout 10 sfirstorder.
+  Qed.
+
+  Lemma may_write_all_expr_log :
+    forall log_r log_a P0 sys input expr dst_sz ops,
+      may_write_all log_r log_a P0 (affected_regs ops) = true ->
+      may_write_all log_r (expr_log expr dst_sz sys input log_a) P0 (affected_regs ops) = true.
+  Proof.
+    intros log_r log_a P0 sys input expr dst_sz ops Hwr.
+    unfold may_write_all in *. rewrite forallb_forall in *. intros reg Hreg_in_aff.
+    specialize (Hwr reg Hreg_in_aff).
+
+    unfold expr_log. induction (snd (eval_expr_aux expr [] sys input)).
+    - exact Hwr.
+    - simpl. destruct (eq_dec reg a) as [Heq | Hneq]; subst.
+      + simpl. rewrite may_write_log_cons_eq. apply andb_true_intro; split.
+        * assumption.
+        * destruct P0; simpl; try reflexivity. destruct a; try ring.
+          contradict Hreg_in_aff. exact (inputs_not_affected ops x).          
+      + simpl. rewrite may_write_log_cons_neq.
+        * apply IHl.
+        * assumption.
+  Qed.
+
+  Lemma may_write_expr_log :
+    forall log_r log_a P0 sys input expr dst_sz reg ,
+      (forall i, tf_in i <> reg) ->
+      may_write log_r log_a P0 reg = true ->
+      may_write log_r (expr_log expr dst_sz sys input log_a) P0 reg = true.
+  Proof.
+    intros log_r log_a P0 sys input expr dst_sz reg Hnot_input Hwr.
+    unfold expr_log. induction (snd (eval_expr_aux expr [] sys input)).
+    - exact Hwr.
+    - simpl. destruct (eq_dec reg a) as [Heq | Hneq]; subst.
+      + simpl. rewrite may_write_log_cons_eq. apply andb_true_intro; split.
+        * assumption.
+        * destruct P0; simpl; try reflexivity. destruct a; try ring.
+          specialize (Hnot_input x). contradiction.
+      + simpl. rewrite may_write_log_cons_neq.
+        * apply IHl.
+        * assumption.
+  Qed.
+    
   Lemma interp_action_aux :
     forall (sys: sys_state_t) (r: ContextEnv.(env_t) R) 
            (act: spec_action) (input: input_t)
            (sigma: forall f, Sig_denote (Sigma f))
            log_r log_a ops rest,
       state_matches sys r ->
-      env_matches act input r ->
+      may_read_all log_r P0 (map tf_reg spec_all_states) = true ->
       may_read_all log_r P1 (map tf_in spec_all_inputs) = true ->
+      may_read_all log_r P0 (map tf_out spec_all_outputs) = true ->
+      inputs_are_buffered input r (log_app log_a log_r) ->
       NoDup (affected_regs ops) ->
       may_write_all log_r log_a P0 (affected_regs ops) = true ->
-      match interp_action (tau:=unit_t) r sigma (CtxReadVars r (map tf_out spec_all_outputs) (rev (map (fun r0 : reg_t => (_register_var_name tf_ctx r0, R r0)) (map tf_reg spec_all_states)) ++ [])
-                                    (CtxReadVars r (map tf_reg spec_all_states) [] CtxEmpty))
-              log_r log_a (rule_aux tf_ctx ops rest)
+      match interp_action (tau:=unit_t) r sigma CtxEmpty log_r log_a (rule_aux tf_ctx ops rest)
       return option (Log R REnv) with
       | Some (l, _, _) => Some (l)
       | None => None
       end =
-      None.
+      match interp_action r sigma CtxEmpty log_r (aux_log sys input ops log_a) rest
+      with
+      | Some (l, _, _) => Some l
+      | None => None
+      end.
   Proof.
-    intros r sigma log_r log_a ops rest.
-    intros Hrd1_in HNoDup_aff Hwr0_aff.
+    intros sys r act input sigma log_r log_a ops rest.
+    intros Hstate Hrd0_st Hrd1_in Hrd0_out Hin_buf HNoDup_aff Hwr0_aff.
 
     generalize dependent log_a. generalize dependent rest.
     induction ops as [| op ops H0 ]; intros.
-    - admit.
+    - reflexivity.
     - destruct op.
-      + cbn. apply H0; [ exact HNoDup_aff | exact Hwr0_aff ].
-      + cbn. cbn in Hwr0_aff. apply may_write_all_cons in Hwr0_aff. destruct Hwr0_aff as [Hwr0_dst Hwr0_rest].
-        admit.
-        (* rewrite Hwr0_dst. apply H0; [| exact Hwr0_rest]. *)
-  Admitted.
+      + cbn. apply H0; assumption.
+      + simpl. simpl in Hwr0_aff. apply may_write_all_cons in Hwr0_aff. destruct Hwr0_aff as [Hwr0_dst Hwr0_rest].
+        unfold opt_bind. 
+        change (@tf_states_type _ (tfs_states_size (tf_sched_ctx tf_ctx)) dst)
+          with (bits_t (tfs_states_size (tf_sched_ctx tf_ctx) dst)) in *.
+        rewrite (interp_action_expr sys r act input sigma log_r log_a expr); try assumption.
+        extract_match_term. assert (MT = true).
+        * subst. apply may_write_expr_log.
+          -- intros. (* hammer. *) timeout 10 sauto.
+          -- assumption.
+        * rewrite H. apply H0; clear H0.   
+          -- simpl in HNoDup_aff. inversion HNoDup_aff; subst. assumption.
+          -- apply inputs_are_buffered_log_app_log_cons_neq; try apply inputs_are_buffered_expr_log; try assumption.
+             exact (not_in_reg_reg_all_inputs dst).
+          -- simpl in HNoDup_aff. inversion HNoDup_aff; subst.
+             rewrite may_write_all_log_cons_neq; [|assumption].
+             apply may_write_all_expr_log; assumption.
+      + simpl. simpl in Hwr0_aff. apply may_write_all_cons in Hwr0_aff. destruct Hwr0_aff as [Hwr0_dst Hwr0_rest].
+        unfold opt_bind. 
+        change (@tf_outputs_type _ (tfs_outputs_size (tf_sched_ctx tf_ctx)) dst)
+          with (bits_t (tfs_outputs_size (tf_sched_ctx tf_ctx) dst)) in *.
+        rewrite (interp_action_expr sys r act input sigma log_r log_a expr); try assumption.
+        extract_match_term. assert (MT = true).
+        * subst. apply may_write_expr_log.
+          -- intros. (* hammer. *) timeout 10 sauto.
+          -- assumption.
+        * rewrite H. apply H0; clear H0.   
+          -- simpl in HNoDup_aff. inversion HNoDup_aff; subst. assumption.
+          -- apply inputs_are_buffered_log_app_log_cons_neq; try apply inputs_are_buffered_expr_log; try assumption.
+             exact (not_in_reg_out_all_inputs dst).
+          -- simpl in HNoDup_aff. inversion HNoDup_aff; subst.
+             rewrite may_write_all_log_cons_neq; [|assumption].
+             apply may_write_all_expr_log; assumption.
+  (* Timeout 10 Time Qed.  *)
+  Admitted. (* SPEEDUP *)
+  (* > 10 seconds *)
 
   Definition construct_log (sys: sys_state_t) (act: spec_action) (input: input_t) ready (log_a: Log R ContextEnv): Log R ContextEnv :=
     let updates := if 
@@ -996,33 +1816,147 @@ Section SynthesisCorrectness.
     | right Hnotready => log_a (* TODO: update while working on the proof below *)
     end.
 
+  Lemma nodup_affected_regs_fst:
+    forall act,
+      NoDup (affected_regs (fst (spec_schedule act))).
+  Proof.
+    intros act. 
+    pose proof (spec_schedule_ops_nodup act). unfold tfs_ops_no_duplicates in *.
+    rewrite flat_map_app in H. apply NoDup_app_remove_r in H.
+
+    induction (fst (spec_schedule act)).
+    - simpl. apply NoDup_nil. 
+    - simpl in *. destruct a.
+      + simpl in H. apply IHl. exact H.
+      + simpl in H. apply NoDup_cons_iff in H. destruct H as [Hnotin H]. specialize (IHl H); clear H. 
+        apply NoDup_cons; try assumption.
+        induction l.
+        * auto.
+        * simpl in *. apply Common.not_in_app_iff in Hnotin. destruct Hnotin as [Hnotin Hnotin_l].
+          specialize (IHl0 Hnotin_l); clear Hnotin_l.          
+          destruct a.
+          -- simpl. apply IHl0. exact IHl.
+          -- simpl. destruct (eq_dec dst dst0) as [Heq | Hneq]; subst.
+              ++ contradict Hnotin. sauto.
+              ++ intro. destruct H.
+              ** timeout 10 sauto.
+              ** inversion IHl; subst. apply IHl0; assumption.
+          -- simpl. intro. destruct H.
+              ** timeout 10 sauto.
+              ** inversion IHl; subst. apply IHl0; assumption.
+      + simpl in H. apply NoDup_cons_iff in H. destruct H as [Hnotin H]. specialize (IHl H); clear H. 
+        apply NoDup_cons; try assumption.
+        induction l.
+        * auto.
+        * simpl in *. apply Common.not_in_app_iff in Hnotin. destruct Hnotin as [Hnotin Hnotin_l].
+          specialize (IHl0 Hnotin_l); clear Hnotin_l.          
+          destruct a.
+          -- simpl. apply IHl0. exact IHl.
+          -- simpl. intro. destruct H.
+              ** timeout 10 sauto.
+              ** inversion IHl; subst. apply IHl0; assumption.
+          -- simpl. destruct (eq_dec dst dst0) as [Heq | Hneq]; subst.
+              ++ contradict Hnotin. sauto.
+              ++ intro. destruct H.
+              ** timeout 10 sauto.
+              ** inversion IHl; subst. apply IHl0; assumption.
+  Qed.
+
+  Lemma nodup_affected_regs_snd:
+    forall act,
+      NoDup (affected_regs (snd (spec_schedule act))).
+  Proof.
+    intros act. 
+    pose proof (spec_schedule_ops_nodup act). unfold tfs_ops_no_duplicates in *.
+    rewrite flat_map_app in H. apply NoDup_app_remove_l in H.
+
+    induction (snd (spec_schedule act)).
+    - simpl. apply NoDup_nil. 
+    - simpl in *. destruct a.
+      + simpl in H. apply IHl. exact H.
+      + simpl in H. apply NoDup_cons_iff in H. destruct H as [Hnotin H]. specialize (IHl H); clear H. 
+        apply NoDup_cons; try assumption.
+        induction l.
+        * auto.
+        * simpl in *. apply Common.not_in_app_iff in Hnotin. destruct Hnotin as [Hnotin Hnotin_l].
+          specialize (IHl0 Hnotin_l); clear Hnotin_l.          
+          destruct a.
+          -- simpl. apply IHl0. exact IHl.
+          -- simpl. destruct (eq_dec dst dst0) as [Heq | Hneq]; subst.
+              ++ contradict Hnotin. sauto.
+              ++ intro. destruct H.
+              ** timeout 10 sauto.
+              ** inversion IHl; subst. apply IHl0; assumption.
+          -- simpl. intro. destruct H.
+              ** timeout 10 sauto.
+              ** inversion IHl; subst. apply IHl0; assumption.
+      + simpl in H. apply NoDup_cons_iff in H. destruct H as [Hnotin H]. specialize (IHl H); clear H. 
+        apply NoDup_cons; try assumption.
+        induction l.
+        * auto.
+        * simpl in *. apply Common.not_in_app_iff in Hnotin. destruct Hnotin as [Hnotin Hnotin_l].
+          specialize (IHl0 Hnotin_l); clear Hnotin_l.          
+          destruct a.
+          -- simpl. apply IHl0. exact IHl.
+          -- simpl. intro. destruct H.
+              ** timeout 10 sauto.
+              ** inversion IHl; subst. apply IHl0; assumption.
+          -- simpl. destruct (eq_dec dst dst0) as [Heq | Hneq]; subst.
+              ++ contradict Hnotin. sauto.
+              ++ intro. destruct H.
+              ** timeout 10 sauto.
+              ** inversion IHl; subst. apply IHl0; assumption.
+  Qed.
+
+  (* Lemma affected_regs_fst_not_in_snd:
+    forall act reg, 
+      In reg (affected_regs (fst (spec_schedule act))) 
+      -> ~ In reg (affected_regs (snd (spec_schedule act))).
+  Proof. *)
+
   Lemma interp_action_cmd :
     forall (sys: sys_state_t) (r: ContextEnv.(env_t) R) 
            (act: spec_action) (input: input_t)
            (sigma: forall f, Sig_denote (Sigma f))
            log_r log_a,
       state_matches sys r ->
-      env_matches act input r ->
       may_read_all log_r P0 (map tf_reg spec_all_states) = true ->
       may_write_all log_r log_a P0 (map tf_reg spec_all_states) = true ->
       may_read_all log_r P1 (map tf_in spec_all_inputs) = true ->
       may_read_all log_r P0 (map tf_out spec_all_outputs) = true ->
       may_write_all log_r log_a P0 (map tf_out spec_all_outputs) = true ->
-      may_write log_r log_a P1 (tf_ready) = true ->
+      inputs_are_buffered input r (log_app log_a log_r) ->
       match interp_action r sigma CtxEmpty log_r log_a (_rule_cmd tf_ctx act) with
       | Some (l, v, _) => Some (l)
       | None => None
       end =
       Some ( construct_log sys act input r.[tf_ready] log_a ).
   Proof.
-    intros sys r act input sigma log_r log_a Hstate Hinput_rdy Hinput_nrdy.
-    intros Hrd0_st Hwr0_st Hrd1_in Hrd0_out Hwr0_out Hwr1_ready.
+    intros sys r act input sigma log_r log_a.
+    intros Hstate Hrd0_st Hwr0_st Hrd1_in Hrd0_out Hwr0_out Hin_buf.
     
-    unfold _rule_cmd. rewrite interp_action_read_vars_states; try assumption.
-    rewrite interp_action_read_vars_outputs; try assumption.
+    unfold _rule_cmd. 
+    rewrite (interp_action_aux sys r act input sigma log_r log_a); try timeout 1 assumption.
+    2: exact (nodup_affected_regs_fst act).
+    2: {
+      unfold affected_regs. 
+      induction (fst (spec_schedule act)).
+      - simpl. unfold may_write_all. rewrite forallb_forall. intros reg Hreg_in_aff. contradiction.
+      - simpl. unfold may_write_all in *. rewrite forallb_forall in *. intros reg Hreg_in_aff. specialize (IHl reg).
+        destruct a.
+        + specialize (IHl Hreg_in_aff). apply IHl.
+        + simpl in Hreg_in_aff. destruct (Hreg_in_aff); clear Hreg_in_aff; subst.
+            * apply Hwr0_st. apply in_map. exact (in_spec_all_states dst).
+            * apply IHl. apply H.
+        + simpl in Hreg_in_aff. destruct (Hreg_in_aff); clear Hreg_in_aff; subst.
+            * apply Hwr0_out. apply in_map. exact (in_spec_all_outputs dst).
+            * apply IHl. apply H.
+    }
+
     admit.
   Admitted.
 
+  (*
   Lemma interp_rule_correct :
     forall (sys: sys_state_t) (r: ContextEnv.(env_t) R) 
            (act: spec_action) (input: input_t)
@@ -1089,12 +2023,83 @@ Section SynthesisCorrectness.
   (* Time Qed. *)
   Admitted. (* SPEEDUP *)
   (* ??? seconds *)
+   *)
+
+  Definition good_log (log: Log R ContextEnv) : Prop :=
+    may_read_all log P0 (map tf_reg spec_all_states) = true /\
+    may_write_all log log_empty P0 (map tf_reg spec_all_states) = true /\
+    may_read_all log P0 (map tf_in spec_all_inputs) = true /\
+    may_write_all log log_empty P0 (map tf_in spec_all_inputs) = true /\
+    may_read_all log P0 (map tf_out spec_all_outputs) = true /\
+    may_write_all log log_empty P0 (map tf_out spec_all_outputs) = true /\
+    may_read log P0 (tf_ready) = true /\
+    may_write log log_empty P0 (tf_ready) = true /\
+    may_read log P0 (tf_cmd) = true /\
+    may_write log log_empty P0 (tf_cmd) = true.
+
+  (* Lemma interp_rule_correct :
+    forall (sys: sys_state_t) (r: ContextEnv.(env_t) R) 
+           (act: spec_action) (input: input_t)
+           (sigma: forall f, Sig_denote (Sigma f))
+           log,
+      state_matches sys r ->
+      ( r.[tf_ready] = Ob~1 -> input_matches act input sigma ) ->
+      ( r.[tf_ready] = Ob~0 -> env_matches act input r ) ->
+      good_log log ->
+      let guard_log := if Bits.single r.[tf_ready] then log_after_cmd_guard_rdy act sigma else log_cons tf_cmd Read0 (log_cons tf_ready Read0 log_empty) in
+      interp_rule r sigma log (rules (rule_cmd act)) = Some (construct_log sys act input r.[tf_ready] guard_log).
+  Proof.
+    intros sys r act input sigma log Hstate Hinput_rdy Hinput_nrdy.
+    intros Hrd0_st Hwr0_st Hrd0_in Hwr0_in Hrd0_out Hwr0_out Hrd0_rdy Hwr0_ready Hrd0_cmd Hwr0_cmd.
+    unfold interp_rule, rules.
+
+    rewrite interp_action_seq. unfold opt_bind.
+    rewrite (interp_action_cmd_guard sys r act input sigma log); try assumption.
+
+    setoid_rewrite (interp_action_cmd sys r act input sigma log 
+              (if Bits.single r.[tf_ready] 
+                then log_after_cmd_guard_rdy act sigma 
+                else log_cons tf_cmd Read0 (log_cons tf_ready Read0 log_empty))).
+    - reflexivity.
+    - assumption.
+    - assumption.
+    - assumption.
+    - assumption.
+    - destruct (reg_ready_or_not r) as [Hready | Hnotready].
+      + rewrite Hready. cbn. unfold log_after_cmd_guard_rdy. 
+        rewrite !may_write_all_log_cons_neq. rewrite may_write_all_fold_cons_w0_inputs. rewrite !may_write_all_log_cons_neq. assumption.
+        all: (try exact not_in_reg_ready_all_states); (try exact not_in_reg_cmd_all_states).
+        intros. rewrite in_map_iff in H. destruct H as [x0 [Heq Hin]]. subst. exact (not_in_reg_reg_all_inputs x0).
+      + rewrite Hnotready. cbn. rewrite !may_write_all_log_cons_neq. assumption.
+        all: (try exact not_in_reg_ready_all_states); (try exact not_in_reg_cmd_all_states).
+    - apply may_read_all0_implies_may_read_all1. assumption.  
+    - assumption.
+    - destruct (reg_ready_or_not r) as [Hready | Hnotready].
+      + rewrite Hready. cbn. unfold log_after_cmd_guard_rdy. 
+        rewrite !may_write_all_log_cons_neq. rewrite may_write_all_fold_cons_w0_inputs. rewrite !may_write_all_log_cons_neq. assumption.
+        all: (try exact not_in_reg_ready_all_outputs); (try exact not_in_reg_cmd_all_outputs).
+        intros. rewrite in_map_iff in H. destruct H as [x0 [Heq Hin]]. subst. exact (not_in_reg_out_all_inputs x0).
+      + rewrite Hnotready. cbn. rewrite !may_write_all_log_cons_neq. assumption.
+        all: (try exact not_in_reg_ready_all_outputs); (try exact not_in_reg_cmd_all_outputs).
+    - destruct (reg_ready_or_not r) as [Hready | Hnotready].
+      + rewrite Hready. cbn. unfold log_after_cmd_guard_rdy.
+        rewrite may_write_log_cons_eq. rewrite may_write_log_cons_neq. 
+        rewrite may_write_fold_cons_w0_inputs. rewrite !may_write_log_cons_eq. simpl. rewrite !andb_true_r.
+        * apply may_write0_implies_may_write1. assumption. 
+        * exact not_in_reg_ready_all_inputs. 
+        * intro. congruence.
+      + rewrite Hnotready. cbn. rewrite may_write_log_cons_neq. rewrite may_write_log_cons_eq. simpl. rewrite !andb_true_r.
+        * apply may_write0_implies_may_write1. assumption.
+        * intro. congruence.
+  (* Time Qed. *)
+  Admitted. (* SPEEDUP *)
+  (* ??? seconds *)
 
   (* 
     Once we can substitue the expensive HW interpretation with a contructed log, we should be able to work on the lemmas below
     until then we do not wish to proceed past this point
   *)
-Abort.
+Abort. *)
 
   Lemma latest_write_cmd_rdy :
     forall (sys: sys_state_t) (r: ContextEnv.(env_t) R) 
@@ -1214,6 +2219,8 @@ Abort.
   Proof.
   Admitted.
 
+  (* Below is done *)
+
   Lemma synthesis_correct_aux3 :
     forall (sys: sys_state_t) (r: ContextEnv.(env_t) R) 
            (act: spec_action) (input: input_t)
@@ -1243,7 +2250,7 @@ Abort.
       + unfold commit_update. rewrite getenv_create.
         destruct (reg_ready_or_not r) as [Hready | Hnotready].
         * rewrite (latest_write_cmd_rdy sys r act input sigma log); try assumption; reflexivity.
-        * rewrite (latest_write_cmd_nrdy sys r act input sigma log); try assumption. apply (Hin_nrdy Hnotready). auto.
+        * rewrite (latest_write_cmd_nrdy sys r act input sigma log); try assumption. apply (Hin_nrdy Hnotready).
       + unfold commit_update. rewrite getenv_create.
         destruct (reg_ready_or_not r) as [Hready | Hnotready].
         * rewrite (latest_write_input_rdy sys r act input sigma log x); try assumption; reflexivity.
@@ -1262,7 +2269,7 @@ Abort.
       interp_rule r sigma log (rules (rule_cmd a)) = None.
   Proof.
     intros sys r act input sigma log a Hstate Hin_rdy Hin_nrdy Hact_neq_a.
-    unfold interp_rule, rules, rule_cmd_guard. simpl_eq. (* Takes a while, but otherwise qed stalls *)
+    unfold interp_rule, rules, rule_cmd_guard. simpl_eq.
     destruct may_read; try reflexivity. timeout 10 cbn. 
     destruct (reg_ready_or_not r) as [Hready | Hnotready].
     - specialize (Hin_rdy Hready) as H_in. rewrite Hready. timeout 10 cbn.
@@ -1313,7 +2320,7 @@ Abort.
           | Some l => interp_scheduler' r sigma rules (log_app l log) (fold_right (fun (t : spec_action) (acc : scheduler) => rule_cmd t |> acc) (system_schedule_outputs tf_ctx) actions)
           | None => interp_scheduler' r sigma rules log (fold_right (fun (t : spec_action) (acc : scheduler) => rule_cmd t |> acc) (system_schedule_outputs tf_ctx) actions)
           end)
-      =
+      <->
       state_env_matches (tfs_next_cycle sched_ctx act sys input) act input (commit_update r
           match interp_rule r sigma log (rules (rule_cmd act)) with
           | Some l => (log_app l log)
@@ -1323,10 +2330,26 @@ Abort.
     intros sys r act input sigma log actions Hstate Hin_rdy Hin_nrdy Hlog H_notin_actions.
 
     induction actions as [|a actions IH].
-    - cbn [fold_right]. 
-      apply state_env_matches_comp;
-        (* All: *) unfold state_equal, env_equal; split;
-          (* All: *) intros x; unfold commit_update; rewrite !getenv_create; match_eq; destruct interp_rule; apply latest_write_schedule_outputs; reflexivity.
+    - cbn [fold_right].
+
+      remember (commit_update r
+                  match interp_rule r sigma log (rules (rule_cmd act)) with
+                  | Some l => interp_scheduler' r sigma rules (log_app l log) (system_schedule_outputs tf_ctx)
+                  | None => interp_scheduler' r sigma rules log (system_schedule_outputs tf_ctx)
+                  end) as r1.
+      remember (commit_update r
+                  match interp_rule r sigma log (rules (rule_cmd act)) with
+                  | Some l => log_app l log
+                  | None => log
+                  end) as r2.
+      assert (state_equal r1 r2) as Heq_s. {
+        subst r1 r2. unfold state_equal, env_equal; split; intros x; unfold commit_update; rewrite !getenv_create; match_eq; destruct interp_rule; apply latest_write_schedule_outputs; reflexivity.
+      }
+      assert (env_equal r1 r2) as Heq_e. {
+        subst r1 r2. unfold state_equal, env_equal; split; try intros x; unfold commit_update; rewrite !getenv_create; match_eq; destruct interp_rule; apply latest_write_schedule_outputs; reflexivity.
+      }
+
+      apply state_env_matches_comp with (r1:=r1) (r2:=r2); try assumption.
     - apply not_in_cons in H_notin_actions. destruct H_notin_actions as [Hneq Hnotin].
 
       cbn [fold_right interp_scheduler'].
@@ -1400,7 +2423,7 @@ Abort.
 
     (* prove we may read *)
     set (mr := may_read _ _ _). assert (mr = true). 
-    { subst mr. unfold may_read. rewrite !SemanticProperties.log_existsb_empty. sauto. }
+    { subst mr. rewrite may_read_log_empty. reflexivity. }
     rewrite H. clear H mr.
     
     unfold opt_bind.
@@ -1409,8 +2432,10 @@ Abort.
     (* prove we may write *)
     set (mw := may_write _ _ _ _). assert (mw = true). 
     { 
-      subst mw. unfold may_write. rewrite !SemanticProperties.log_existsb_app. rewrite !Common.log_existsb_cons. rewrite !SemanticProperties.log_existsb_empty.
-      (* hammer *) timeout 10 hauto.
+      subst mw. rewrite !may_write_log_cons_neq.
+      - rewrite may_write_log_empty. reflexivity.
+      - sauto.
+      - sauto.
     }
     rewrite H, Hready. reflexivity.
   Qed.
@@ -1438,8 +2463,10 @@ Abort.
       rewrite H_busy_ready. clear H_busy_ready.
 
       apply synthesis_correct_aux; try assumption.
+
       (* Show that the log is good *)
-      exact log_empty_good_log.
+      unfold good_log. repeat split; try apply may_read_all_log_empty; try apply may_write_all_log_empty; 
+      try apply may_read_log_empty; try apply may_write_log_empty.
 
     - specialize (Hin_nrdy Hnotready) as H_in.
 
@@ -1448,10 +2475,55 @@ Abort.
       rewrite H_busy_not_ready. clear H_busy_not_ready.
 
       apply synthesis_correct_aux; try assumption.
+
       (* Show that the log is good *)
-      apply good_log_app; try exact log_empty_good_log.
-      apply good_log_cons. apply good_log_cons. apply good_log_cons.
-      all: try exact log_empty_good_log; try timeout 10 sauto.
+      unfold good_log. repeat split.
+      + rewrite !SemanticProperties.log_app_empty_l. rewrite !may_read_all_log1_cons_neq.
+        * apply may_read_all_log_empty.
+        * exact not_in_reg_ready_all_states.
+        * exact not_in_reg_ready_all_states.
+        * exact not_in_reg_cmd_ack_all_states.
+      + rewrite !SemanticProperties.log_app_empty_l. rewrite !may_write_all_log1_cons_neq.
+        * apply may_write_all_log_empty.
+        * exact not_in_reg_ready_all_states.
+        * exact not_in_reg_ready_all_states.
+        * exact not_in_reg_cmd_ack_all_states.
+      + rewrite !SemanticProperties.log_app_empty_l. rewrite !may_read_all_log1_cons_neq.
+        * apply may_read_all_log_empty.
+        * exact not_in_reg_ready_all_inputs.
+        * exact not_in_reg_ready_all_inputs.
+        * exact not_in_reg_cmd_ack_all_inputs.
+      + rewrite !SemanticProperties.log_app_empty_l. rewrite !may_write_all_log1_cons_neq.
+        * apply may_write_all_log_empty.
+        * exact not_in_reg_ready_all_inputs.
+        * exact not_in_reg_ready_all_inputs.
+        * exact not_in_reg_cmd_ack_all_inputs.
+      + rewrite !SemanticProperties.log_app_empty_l. rewrite !may_read_all_log1_cons_neq.
+        * apply may_read_all_log_empty.
+        * exact not_in_reg_ready_all_outputs.
+        * exact not_in_reg_ready_all_outputs.
+        * exact not_in_reg_cmd_ack_all_outputs.
+      + rewrite !SemanticProperties.log_app_empty_l. rewrite !may_write_all_log1_cons_neq.
+        * apply may_write_all_log_empty.
+        * exact not_in_reg_ready_all_outputs.
+        * exact not_in_reg_ready_all_outputs.
+        * exact not_in_reg_cmd_ack_all_outputs.
+      + rewrite !SemanticProperties.log_app_empty_l. rewrite may_read_log1_cons_neq. rewrite !may_read_log1_cons_eq.
+        * rewrite may_read_log_empty. ring.
+        * sauto.
+      + rewrite !SemanticProperties.log_app_empty_l. rewrite may_write_log1_cons_neq. rewrite !may_write_log1_cons_eq.
+        * rewrite may_write_log_empty. ring.
+        * sauto.
+      + rewrite !SemanticProperties.log_app_empty_l. rewrite !may_read_log1_cons_neq.
+        * apply may_read_log_empty.
+        * sauto.
+        * sauto.
+        * sauto.
+      + rewrite !SemanticProperties.log_app_empty_l. rewrite !may_write_log1_cons_neq.
+        * apply may_write_log_empty.
+        * sauto.
+        * sauto.
+        * sauto.
   Qed.
 
 End SynthesisCorrectness.
